updating

SF_calculus/SF_size.v.d
@@ -1,2 +1,2 @@
-SF_calculus/SF_size.vo SF_calculus/SF_size.glob SF_calculus/SF_size.v.beautified: SF_calculus/SF_size.v SF_calculus/General.vo SF_calculus/SF_Terms.vo SF_calculus/SF_Tactics.vo SF_calculus/SF_reduction.vo SF_calculus/SF_Normal.vo SF_calculus/SF_Closed.vo SF_calculus/Substitution.vo SF_calculus/SF_Eval.vo SF_calculus/Star.vo SF_calculus/Fixpoints.vo SF_calculus/Extensions.vo SF_calculus/Tagging.vo SF_calculus/Adding.vo
-SF_calculus/SF_size.vio: SF_calculus/SF_size.v SF_calculus/General.vio SF_calculus/SF_Terms.vio SF_calculus/SF_Tactics.vio SF_calculus/SF_reduction.vio SF_calculus/SF_Normal.vio SF_calculus/SF_Closed.vio SF_calculus/Substitution.vio SF_calculus/SF_Eval.vio SF_calculus/Star.vio SF_calculus/Fixpoints.vio SF_calculus/Extensions.vio SF_calculus/Tagging.vio SF_calculus/Adding.vio
+SF_size.vo SF_size.glob SF_size.v.beautified: SF_size.v
+SF_size.vio: SF_size.v
