Fieska_calculus/Adding.v
@@ -45,13 +45,13 @@ Ltac unfold_op := unfold s_op2, a_op, i_op, id, k_op, f_op, s_op.
 Lemma s_op2_normal: forall M N, normal M -> normal N -> normal (App (App (Op Sop) M) N).
 Proof. intros; nf_out. Qed. 
 
-Lemma k_op_normal: forall M, normal M -> normal (App (App (Op Fop) (Op Fop)) M).
+Lemma k_op_normal: forall M, normal M -> normal (App (Op Kop) M).
 Proof. intros;  nf_out. Qed. 
 
 Ltac nf_out2 := 
 match goal with 
 | |- normal (App (App (Op Sop) _) _) => apply s_op2_normal; nf_out2
-| |- normal (App (App (Op Fop) (Op Fop)) _) => apply k_op_normal; nf_out2
+| |- normal (App (Op Kop) _) => apply k_op_normal; nf_out2
 | _ => nf_out
 end. 
 
@@ -132,59 +132,285 @@ add sigma i traverses sigma, looking for i.
 
 *) 
 
-Definition add_fn := star_opt (star_opt (* recursion argument and sigma *) 
+
+Definition swap M N := App (App (Op Sop) (App (Op Aop) M)) (App (Op Kop) N).
+
+
+Definition add_fn := star_opt (star_opt (star_opt 
+(* recursion argument, (sigma,x) u  *) 
 (* tag *) 
-(extension (App (App (Op Aop) (App (App (Op Aop) (App (App (Op Aop) (Y_k 3)) (Ref 2))) 
-(Ref 1))) (Ref 0)) 
-           (App (App (App (App (Op Aop) (Ref 4)) (Ref 3)) (Ref 1))
-                (App (App (App (Op Aop) (Ref 4)) (Ref 3)) (Ref 0)))
+(extension (App (App (Op Aop)(App (App (Op Aop)(App (App (Op Aop) (Y_k 3)) (Ref 2))) (Ref 1))) (Ref 0)) 
+        (App (App (App (App (Op Aop) (App (App (Op Aop) (Ref 5)) (Ref 4))) (Ref 3)) (Ref 1))
+             (App (App (App (Op Aop) (App (App (Op Aop) (Ref 5)) (Ref 4)) )(Ref 3)) (Ref 0)))
 (* var *) 
-(extension (App (App (Op Aop)  (App (App (Op Aop) (Y_k 3)) var_fn)) (Ref 0))
+(extension (App (App (Op Aop) (App (App (Op Aop)(Y_k 3)) (Ref 1))) (Ref 0))  (* var y *) 
                      (App (App (App (App (Op Eop) (Ref 0)) 
-                                    (snd_projection (fst_projection (Ref 1)))) (* x *) 
-                               (snd_projection (Ref 1))) (* u *) 
-                          (App (fst_projection (fst_projection (Ref 1)))  (* sigma *) 
-                               (App (App (Op Aop)  (App (App (Op Aop) (Y_k 3)) var_fn)) (Ref 0))))
-(* abs *)
-(extension (App (App (Op Aop)  (App (App (Op Aop)  
-(App (App (Op Aop)  (App (App (Op Aop) (Ref 5)) (Ref 4))) (Ref 3))) (s_op2 (Ref 2) (Ref 1))))
-(Ref 0))
-           (App (App (Op Aop)  (App (App (Op Aop)  (App (App (Op Aop)  
-(App (App (Op Aop)  (Ref 5)) (Ref 4))) (Ref 3)))
-                                         (s_op2 (App (App (App (Op Aop) (Ref 7)) (Ref 6)) (Ref 2)) (Ref 1))))
-                               (Ref 0))
+                                     (snd_projection (Ref 3))) (* y = x *) 
+                               (Ref 2))  (* u *) 
+                          (App (fst_projection (Ref 3)) 
+                               (App (App (Op Aop) (App (App (Op Aop)(Y_k 3)) (Ref 1)) )(Ref 0))))
+                                          (* sigma (var y) *) 
 (* add  *) 
-(extension (App (App (Op Aop) (Ref 3)) 
-                (App (App (Op Sop) (App (App (Op Sop) (Ref 2)) (Ref 1))) (Ref 0)))
-           (App (App (Op Aop) (Ref 3)) 
-                (App (App (Op Sop) 
-                (App (App (Op Sop) (App (App (App (Op Aop) (Ref 5)) (Ref 4)) (Ref 2))) (Ref 1)))
-                (App (App (App (Op Aop) (Ref 5)) (Ref 4)) (Ref 0))))
-(* Nil *) 
-(fst_projection (fst_projection (Ref 0)))))))).
+(* | Add i u sigma => App (App (Op Aop) add) (s_op2 (s_op2 (lambda_to_fieska sigma) (ref i)) (lambda_to_fieska u))
+*) 
+(extension (App (App (Op Aop) (App (App (Op Aop) (App (App (Op Aop) (Y_k 4)) 
+                                                      (Ref 2)))
+                                   (Ref 1)))
+           (Ref 0))
+  (* add (sigma2, x2) u *) 
+   (App (App (Op Aop) (App (App (Op Aop) (App (App (Op Aop) (Y_k 4)) (Ref 2)))
+     (s_op2 (App (App (App (Op Aop) (App (App (Op Aop) (Ref 5)) 
+                                         (Ref 4))) 
+                      (Ref 3)) 
+                 (fst_projection (Ref 1)))
+        (snd_projection (Ref 1)))))
+     (App (App (App (Op Aop) (App (App (Op Aop) (Ref 5)) (Ref 4))) (Ref 3)) (Ref 0)))
+(* abs = swap (App (App (Op Aop) add (s_op2 sigma x)) t *) 
+(extension (swap (App (App (Op Aop) (Ref 3)) (App (App (Op Sop) (Ref 2)) (Ref 1))) (Ref 0))
+           (swap (App (App (Op Aop) (Ref 3)) (App (App (Op Sop) 
+                                             (App (App (App (Op Aop) 
+                                                            (App (App (Op Aop) (Ref 6))
+                                                                 (Ref 5)))
+                                                       (Ref 4)) 
+                                                  (Ref 2)))
+                                                  (Ref 1)))
+                 (Ref 0))
+(* dummy case *) 
+(fst_projection (Ref 1))
+)))))). 
 
-Definition add :=  App (App (Op Aop) (Y_k 3)) add_fn.
+Definition add :=  App (App (Op Aop) (Y_k 4)) add_fn.
+
+
+Definition abs sigma x t := swap (App (App (Op Aop) add) (s_op2 sigma x)) t .
 
 
 
-Definition abs_fn := star_opt  (* rec'n argument *) 
-(extension (App (App s_op (Ref 1)) (Ref 0)) (* y::ys *) 
-           (star_opt (star_opt (star_opt (* sigma_x t u *) 
-             (App (App (Op Aop)  (App (App (Op Aop)  (App (App (Op Aop)  (Ref 5)) (Ref 3))) 
-                                 (s_op2 (App (App (Op Aop) add) (s_op2 (Ref 2) (Ref 0))) (Ref 4))))
-                       (Ref 1)))))
-           (App k_op (star_opt (star_opt (star_opt (App (App (App (Op Aop) add) 
-                                                        (s_op2 (Ref 2) (Ref 0))) 
-                                                        (Ref 1)))))))
-.
-
-Definition abs xs sigma_x t := 
-  App (App (Op Aop)  (App (App (Op Aop)  (App (App (Op Aop)  
-  (App (App (Op Aop) (Y_k 4)) abs_fn)) xs)) sigma_x)) t. 
+Lemma abs_red : 
+forall sigma x t u, sf_red (App (abs sigma x t) u) 
+                           (App (App (App (Op Aop) (App (App (Op Aop) add) (s_op2 sigma x)))
+                                      u) t). 
+Proof.
+intros; unfold abs, swap; unfold_op. eval_tac. 
+eapply2 preserves_app_sf_red. eval_tac. 
+Qed. 
 
 
-Lemma add_fn_closed: maxvar add_fn = 0. 
-Proof. cbv. auto. Qed. 
+Lemma add_closed: maxvar add = 0.
+Proof.
+unfold add. unfold maxvar; fold maxvar. rewrite Y_k_closed. unfold max. 
+unfold add_fn. rewrite ! maxvar_star_opt. 
+cbv.  auto. 
+Qed. 
+
+
+
+
+Lemma add_red_tag: 
+forall sigma_x u M N, sf_red (App (App (App add sigma_x) u) (tag M N)) 
+                         (App (App (App (App (Op Aop) (App (App (Op Aop) add) sigma_x)) u) M)
+                              (App (App (App (Op Aop) (App (App (Op Aop) add) sigma_x)) u) N)).
+Proof.
+intros. unfold add at 1. eval_tac. 
+eapply transitive_red. eapply2 Y4_fix. 
+replace (App (App (Op Aop) (Y_k 4)) add_fn) with add by auto. 
+unfold add_fn.
+eapply transitive_red. 
+eapply preserves_app_sf_red. 
+eapply2 star_opt_beta3.  auto. 
+unfold subst; rewrite ! subst_rec_preserves_extension. 
+eapply transitive_red. 
+ eapply2 extensions_by_matching.
+unfold tag, tag_fix.  unfold_op. 
+eapply2 match_app. eapply2 match_app.  
+eapply2 match_app. eapply2 match_app. 
+eapply2 match_app. eapply2 program_matching. 
+unfold program; auto. 
+(* 1 *)  
+unfold map, app, length, fold_left, subst.
+unfold pattern_size; fold pattern_size.
+rewrite ! (pattern_size_closed (Y_k _)). 
+2: apply Y_k_closed. 
+ unfold plus; fold plus. 
+repeat (unfold subst_rec; fold subst_rec; insert_Ref_out). 
+unfold lift. rewrite ! lift_rec_lift_rec; try omega. unfold plus. 
+repeat (rewrite subst_rec_ref; insert_Ref_out; unfold pred). 
+unfold lift. 
+rewrite ! subst_rec_lift_rec; try omega.
+rewrite ! lift_rec_null. auto. 
+Qed. 
+  
+
+
+Lemma add_red_var_unequal: 
+forall i u sigma j, program i -> program j -> i <> j -> 
+sf_red (App (App (App add (s_op2 sigma i)) u) (var j)) (App sigma (var j)).       
+Proof.
+intros. unfold_op;  unfold add at 1. eval_tac. 
+eapply transitive_red. eapply2 Y4_fix. 
+replace (App (App (Op Aop) (Y_k 4)) add_fn) with add by auto. 
+unfold add_fn.
+eapply transitive_red. 
+eapply preserves_app_sf_red. 
+eapply2 star_opt_beta3.  auto. 
+unfold subst; rewrite ! subst_rec_preserves_extension. 
+eapply transitive_red. eapply2 extensions_by_matchfail.
+unfold var, var_fix, var_fn; unfold_op. 
+eapply2 matchfail_compound_l. eapply2 matchfail_compound_r. 
+eapply2 matchfail_compound_l. eapply2 matchfail_compound_r.
+eapply2 matchfail_compound_l. 
+eapply2 matchfail_compound_r. unfold_op; auto. 
+ eapply2 matchfail_compound_l. 
+eapply2 matchfail_compound_l. 
+unfold_op.  
+eapply2 matchfail_op. unfold factorable. left; eauto. discriminate.
+(* 1 *)  
+eapply transitive_red. eapply2 extensions_by_matching.
+unfold var, var_fix; unfold_op. 
+eapply2 match_app. eapply2 match_app. eapply2 match_app. 
+apply program_matching. 
+unfold program; split. nf_out.  auto. 
+(* 1 *) 
+unfold map, app, length, fold_left, subst. 
+unfold pattern_size; fold pattern_size.
+rewrite ! pattern_size_closed; auto.  unfold plus; fold plus. 
+rewrite ! subst_rec_app. rewrite ! subst_rec_op.  
+rewrite ! subst_rec_preserves_snd_projection. 
+rewrite ! subst_rec_preserves_fst_projection. 
+unfold lift. rewrite ! lift_rec_null.
+repeat (rewrite subst_rec_ref at 1; insert_Ref_out). 
+unfold lift; rewrite ! lift_rec_lift_rec; try omega. unfold plus. 
+rewrite ! subst_rec_lift_rec; try omega.
+rewrite ! lift_rec_null.
+unfold subst_rec; fold subst_rec. 
+rewrite ! (subst_rec_closed (Y_k _)); try (rewrite Y_k_closed; omega). 
+eapply transitive_red. eapply preserves_app_sf_red. eapply preserves_app_sf_red. 
+eapply preserves_app_sf_red. auto. 
+eapply2 snd_out. auto.   
+eapply transitive_red. eapply preserves_app_sf_red. eapply2 fst_out. auto. auto. 
+eapply transitive_red. eapply preserves_app_sf_red. eapply preserves_app_sf_red.
+eapply2 unequal_programs. auto. auto. 
+eval_tac. 
+Qed.
+
+Lemma add_red_var_equal: 
+forall i u sigma, program i -> 
+sf_red (App (App (App add (s_op2 sigma i)) u) (var i)) u.       
+Proof.
+intros. unfold_op;  unfold add at 1. eval_tac. 
+eapply transitive_red. eapply2 Y4_fix. 
+replace (App (App (Op Aop) (Y_k 4)) add_fn) with add by auto. 
+unfold add_fn.
+eapply transitive_red. 
+eapply preserves_app_sf_red. 
+eapply2 star_opt_beta3.  auto. 
+unfold subst; rewrite ! subst_rec_preserves_extension. 
+eapply transitive_red. eapply2 extensions_by_matchfail.
+unfold var, var_fix, var_fn; unfold_op. 
+eapply2 matchfail_compound_l. eapply2 matchfail_compound_r. 
+eapply2 matchfail_compound_l. eapply2 matchfail_compound_r.
+eapply2 matchfail_compound_l. 
+eapply2 matchfail_compound_r. unfold_op; auto. 
+ eapply2 matchfail_compound_l. 
+eapply2 matchfail_compound_l. 
+unfold_op.  
+eapply2 matchfail_op. unfold factorable. left; eauto. discriminate.
+(* 1 *)  
+eapply transitive_red. eapply2 extensions_by_matching.
+unfold var, var_fix; unfold_op. 
+eapply2 match_app. eapply2 match_app. eapply2 match_app. 
+apply program_matching. 
+unfold program; split. nf_out.  auto. 
+(* 1 *) 
+unfold map, app, length, fold_left, subst. 
+unfold pattern_size; fold pattern_size.
+rewrite ! pattern_size_closed; auto.  unfold plus; fold plus. 
+rewrite ! subst_rec_app. rewrite ! subst_rec_op.  
+rewrite ! subst_rec_preserves_snd_projection. 
+rewrite ! subst_rec_preserves_fst_projection. 
+unfold lift. rewrite ! lift_rec_null.
+repeat (rewrite subst_rec_ref at 1; insert_Ref_out). 
+unfold lift; rewrite ! lift_rec_lift_rec; try omega. unfold plus. 
+rewrite ! subst_rec_lift_rec; try omega.
+rewrite ! lift_rec_null.
+unfold subst_rec; fold subst_rec. 
+rewrite ! (subst_rec_closed (Y_k _)); try (rewrite Y_k_closed; omega). 
+eapply transitive_red. eapply preserves_app_sf_red. eapply preserves_app_sf_red. 
+eapply preserves_app_sf_red. auto. 
+eapply2 snd_out. auto.   
+eapply transitive_red. eapply preserves_app_sf_red. eapply2 fst_out. auto. auto. 
+eapply transitive_red. eapply preserves_app_sf_red. eapply preserves_app_sf_red.
+eapply2 equal_programs. auto. auto. 
+eval_tac. 
+Qed.
+
+
+Lemma subst_rec_preserves_swap: 
+forall M N P k, subst_rec (swap M N) P k = swap (subst_rec M P k) (subst_rec N P k).
+Proof. intros; unfold swap, subst_rec; auto. Qed. 
+
+Lemma pattern_size_swap: 
+forall M N, pattern_size(swap M N) = pattern_size M + pattern_size N. 
+Proof. intros; unfold swap, pattern_size; fold pattern_size; omega.  Qed. 
+
+
+Lemma add_red_abs : 
+forall sigma x t sigma_y u, 
+  sf_red (App (App (App add sigma_y) u) (abs sigma x t))
+         (abs (App (App (App (Op Aop) (App (App (Op Aop) add) sigma_y)) u) sigma) x t). 
+Proof.
+intros. unfold add at 1. eval_tac. 
+eapply transitive_red. eapply2 Y4_fix. 
+replace (App (App (Op Aop) (Y_k 4)) add_fn) with add by auto. 
+unfold add_fn.
+eapply transitive_red. 
+eapply preserves_app_sf_red. 
+eapply2 star_opt_beta3.  auto. 
+unfold subst; rewrite ! subst_rec_preserves_extension. 
+eapply transitive_red. eapply2 extensions_by_matchfail.
+unfold abs, swap; unfold_op; auto. 
+eapply2 matchfail_compound_l. 
+eapply2 matchfail_compound_l. 
+eapply2 matchfail_op. 
+unfold factorable; eauto. discriminate. 
+(* 1 *) 
+eapply  transitive_red. 
+eapply2 extensions_by_matchfail.
+unfold abs, swap; unfold_op; auto. 
+eapply2 matchfail_compound_l. 
+eapply2 matchfail_compound_l. 
+eapply2 matchfail_op. 
+unfold factorable; eauto. discriminate. 
+(* 1 *) 
+eapply  transitive_red. 
+eapply2 extensions_by_matchfail.
+unfold abs, swap; unfold_op; auto. 
+eapply2 matchfail_compound_l. 
+eapply2 matchfail_compound_l. 
+eapply2 matchfail_op. 
+unfold factorable; eauto. discriminate. 
+(* 1 *) 
+eapply  transitive_red. 
+eapply2 extensions_by_matching.
+unfold abs, swap; unfold_op; auto. 
+do 20 eapply2 match_app. 
+unfold map, app, length, fold_left, subst.  
+(* 1 *) 
+ unfold abs. rewrite ! subst_rec_preserves_swap. 
+rewrite ! pattern_size_swap. 
+unfold pattern_size; fold pattern_size. 
+unfold lift; rewrite ! lift_rec_null. unfold plus. 
+rewrite ! lift_rec_lift_rec; try omega. unfold plus; fold plus. 
+repeat (unfold subst_rec; fold subst_rec; insert_Ref_out). 
+unfold lift; rewrite ! lift_rec_null. 
+rewrite ! lift_rec_lift_rec; try omega. unfold plus. 
+rewrite ! subst_rec_lift_rec; try omega. 
+rewrite ! lift_rec_null. 
+auto. 
+Qed.   
+
+
+
 
 
 Lemma add_fn_normal: normal add_fn. 
@@ -192,375 +418,131 @@ Proof.
 unfold add_fn. unfold_op. 
 repeat apply star_opt_normal. 
 unfold fst_projection, snd_projection, left_projection, right_projection. 
-cbv; nf_out; repeat (eapply2 nf_active; nf_out).
+cbv; nf_out; repeat (eapply2 nf_active; nf_out); auto.
 Qed. 
 
-Lemma abs_many_red : 
-forall x1 xs sigma_x t u, sf_red (App (abs (App (App s_op x1) xs) sigma_x t) u)
-                                      (abs xs (s_op2 (App (App (Op Aop) add) (s_op2 sigma_x u)) x1) t).
-Proof.
-intros; unfold abs, abs_fn, s_op2; unfold_op. 
-eapply succ_red. eapply2 a_red. 
-eapply transitive_red. eapply preserves_app_sf_red. eapply succ_red. eapply a_red. auto. auto. auto. 
-eapply transitive_red. eapply preserves_app_sf_red. eapply succ_red. eapply a_red. auto. auto. auto.
-eapply transitive_red. eapply preserves_app_sf_red. eapply succ_red. eapply a_red. auto. auto. auto.
-auto. auto. auto. auto. 
-eapply transitive_red. eapply Y4_fix. 
-eapply transitive_red. eapply preserves_app_sf_red.  eapply preserves_app_sf_red.  
-eapply preserves_app_sf_red.  
-eapply2 star_opt_beta. auto. auto. auto. 
-unfold subst. rewrite subst_rec_preserves_extension. 
-eapply transitive_red. eapply preserves_app_sf_red.  eapply preserves_app_sf_red.  
-eapply extensions_by_matching. 
-eapply match_app; nf_out. auto. auto. 
-unfold map, app, length, fold_left, subst.  
-repeat (rewrite subst_rec_preserves_star_opt at 1). auto. auto. 
-eapply transitive_red.  eapply2 star_opt_beta3.
-unfold pattern_size; fold pattern_size. unfold plus; fold plus. 
-unfold subst; rewrite 6? subst_rec_preserves_app at 1. rewrite 6? subst_rec_preserves_app at 1.  
-repeat (unfold subst_rec; fold subst_rec; insert_Ref_out; unfold pred). 
-unfold lift; rewrite ! lift_rec_lift_rec; try omega. rewrite ! lift_rec_null. unfold plus; fold plus. 
-unfold lift; rewrite ! subst_rec_lift_rec; try omega. rewrite ! lift_rec_null.
-auto. 
+  
+Lemma add_normal: normal add. 
+Proof. 
+unfold add. nf_out. apply add_fn_normal. 
 Qed. 
 
+Lemma abs_normal: 
+forall sigma x t, normal sigma -> normal x -> normal t -> normal (abs sigma x t).  
+Proof. 
+intros. unfold abs, swap. nf_out. 
+eapply2 add_normal. auto. auto. auto.  unfold_op; auto. 
+Qed. 
 
-Lemma abs_red : 
-forall sigma_x t u, sf_red (App (abs s_op sigma_x t) u) 
-                           (App (App (App (Op Aop) add) (s_op2 sigma_x u)) t). 
+Lemma add_red_add: 
+forall sigma_x u sigma2 y v, 
+sf_red (App (App (App add sigma_x) u) (App (App (Op Aop) 
+(App (App (Op Aop) add) (s_op2 sigma2 y))) v))  
+        (App (App (Op Aop) (App (App (Op Aop) add) 
+(s_op2 (App (App (App (Op Aop) (App (App (Op Aop) add) sigma_x)) u) sigma2) y)))
+        (App (App (App (Op Aop) (App (App (Op Aop) add) sigma_x)) u) v)). 
 Proof.
-intros; unfold abs, abs_fn; unfold_op. 
-eapply succ_red. eapply2 a_red. 
-eapply transitive_red. eapply preserves_app_sf_red. eapply succ_red. eapply a_red. auto. auto. auto. 
-eapply transitive_red. eapply preserves_app_sf_red. eapply succ_red. eapply a_red. auto. auto. auto. 
-eapply transitive_red. eapply preserves_app_sf_red. eapply succ_red. eapply a_red. auto. auto. auto. 
-auto. auto. auto. auto. auto. auto. 
+intros. unfold_op;  unfold add at 1. eval_tac. 
+eapply transitive_red. eapply2 Y4_fix. 
+replace (App (App (Op Aop) (Y_k 4)) add_fn) with add by auto. 
+unfold add_fn.
+eapply transitive_red. 
+eapply preserves_app_sf_red. 
+eapply2 star_opt_beta3.  auto. 
+unfold subst; rewrite ! subst_rec_preserves_extension. 
+(* not a tag *) 
+eapply transitive_red. apply extensions_by_matchfail.
+unfold add, add_fn; unfold_op; auto. 
+eapply2 matchfail_compound_l. 
+eapply2 matchfail_compound_r. 
+eapply2 matchfail_compound_l. 
+eapply2 matchfail_compound_r. 
+eapply2 matchfail_compound_l. 
+eapply2 matchfail_compound_r. 
+eapply2 matchfail_compound_l.
+eapply2 matchfail_compound_r. unfold_op; auto. 
+unfold_op. eapply2 matchfail_compound_l. 
+eapply2 matchfail_compound_r.
+eapply2 matchfail_compound_r. 
+eapply2 matchfail_compound_r. 
+eapply2 matchfail_compound_r. 
+eapply2 matchfail_op.  unfold factorable. right; auto.  discriminate. 
+(* 1  not a var *) 
+eapply transitive_red. eapply2 extensions_by_matchfail.
+unfold add; unfold_op; auto. 
+eapply2 matchfail_compound_l. 
+eapply2 matchfail_compound_r. 
+eapply2 matchfail_compound_l. 
+eapply2 matchfail_compound_r. 
+eapply2 matchfail_compound_l. 
+eapply2 matchfail_compound_r; unfold_op. auto.   
+eapply2 matchfail_compound_l.
+eapply2 matchfail_compound_l. unfold_op. 
+eapply2 matchfail_op. unfold factorable. left; eauto. discriminate. 
 (* 1 *) 
-eapply transitive_red. eapply preserves_app_sf_red. eapply Y4_fix. auto. 
-eapply transitive_red. eapply preserves_app_sf_red.  eapply preserves_app_sf_red.  
-eapply preserves_app_sf_red.  eapply preserves_app_sf_red. 
-eapply2 star_opt_beta. auto. auto. auto. auto. 
-unfold subst. rewrite subst_rec_preserves_extension. 
-eapply transitive_red. eapply preserves_app_sf_red.  eapply preserves_app_sf_red.  
-eapply preserves_app_sf_red.  eapply extensions_by_matchfail. 
-eapply matchfail_compound_op; nf_out. auto. auto. auto. 
-rewrite ? subst_rec_app. 
-rewrite ? subst_rec_op. 
-rewrite ? subst_rec_preserves_star_opt. 
-(* 1 *)  
-eapply transitive_red. eapply preserves_app_sf_red. eapply preserves_app_sf_red. 
- eapply preserves_app_sf_red. eapply succ_red. eapply2 k_red. auto. auto. auto. auto. 
-eapply transitive_red. eapply star_opt_beta3. 
-unfold subst. (rewrite 12? subst_rec_preserves_app at 1). 
-unfold subst_rec; fold subst_rec. insert_Ref_out. 
-unfold subst_rec; fold subst_rec. insert_Ref_out.  unfold pred.
-rewrite 4 ? (subst_rec_closed act) at 1; try (rewrite act_closed; omega). 
-unfold subst_rec; fold subst_rec. insert_Ref_out.  
-unfold lift.  
-rewrite ? lift_rec_lift_rec; try omega. unfold plus; fold plus. 
-rewrite ? subst_rec_lift_rec; try omega.
-rewrite ? lift_rec_null; try omega.
-unfold subst_rec; fold subst_rec. insert_Ref_out.  unfold lift; rewrite lift_rec_null. 
-auto. 
+(* 1 add vs add *) 
+eapply transitive_red. eapply2 extensions_by_matching.
+eapply2 match_app. eapply2 match_app. eapply2 match_app.
+eapply2 match_app.  eapply2 match_app.
+eapply2 program_matching.  split; auto. 
+(* 1 *) 
+rewrite ! app_nil_r. 
+replace (length nil) with 0 by auto. 
+rewrite ! map_lift0. 
+unfold map; fold map. 
+unfold fold_left; fold fold_left. 
+unfold app; fold app. 
+unfold_op; unfold pattern_size; fold pattern_size. unfold plus; fold plus.
+rewrite ! pattern_size_closed; try (rewrite Y_k_closed; omega). 
+unfold plus; fold plus.   
+unfold length; fold length. 
+rewrite ! subst_rec_app. rewrite ! subst_rec_op. 
+rewrite ! (subst_rec_closed (Y_k _)); try (rewrite Y_k_closed; omega).
+unfold subst; rewrite ! subst_rec_app.  rewrite ! subst_rec_op. 
+rewrite ! (subst_rec_closed (Y_k _)); try (rewrite Y_k_closed; omega).
+repeat (rewrite subst_rec_ref; insert_Ref_out). 
+ unfold lift; rewrite ! lift_rec_lift_rec; try omega. unfold plus. 
+rewrite ! subst_rec_lift_rec; try omega. 
+rewrite ! lift_rec_null. 
+rewrite ! subst_rec_preserves_snd_projection. 
+rewrite ! subst_rec_preserves_fst_projection. 
+repeat (unfold subst_rec; fold subst_rec; insert_Ref_out). 
+ unfold lift; rewrite ! lift_rec_lift_rec; try omega. unfold plus. 
+rewrite ! subst_rec_lift_rec; try omega. 
+rewrite ! lift_rec_null.
+(* 1 *) 
+eapply2 preserves_app_sf_red. unfold_op. 
+eapply2 preserves_app_sf_red. eapply2 preserves_app_sf_red. 
+eapply2 preserves_app_sf_red. eapply2 preserves_app_sf_red. 
+eapply2 preserves_app_sf_red. unfold_op. eapply2 fst_out. eapply2 snd_out. 
 Qed. 
 
 
 Lemma add_red_empty: 
 forall sigma x u, 
-sf_red (App (App add (s_op2 (s_op2 sigma x) u)) (Op Iop)) (App sigma (Op Iop)) .
+sf_red (App (App (App add (s_op2 sigma x)) u) i_op) (App sigma i_op) .
 Proof.
 intros. unfold_op;  unfold add at 1. eval_tac. 
-eapply transitive_red. eapply2 Y3_fix. 
-replace (App (App (Op Aop) (Y_k 3)) add_fn) with add by auto. 
+eapply transitive_red. eapply2 Y4_fix. 
+replace (App (App (Op Aop) (Y_k 4)) add_fn) with add by auto. 
 unfold add_fn.
 eapply transitive_red. 
 eapply preserves_app_sf_red. 
-eapply2 star_opt_beta2.  auto. 
+eapply2 star_opt_beta3.  auto. 
 unfold subst; rewrite ! subst_rec_preserves_extension. 
 eapply transitive_red. eapply2 extensions_by_matchfail.
 eapply transitive_red. eapply2 extensions_by_matchfail.
 eapply transitive_red. eapply2 extensions_by_matchfail.
 eapply transitive_red. eapply2 extensions_by_matchfail.
+unfold swap; auto. 
 rewrite ! subst_rec_preserves_fst_projection. 
-unfold subst_rec; fold subst_rec. insert_Ref_out.
-unfold lift. rewrite lift_rec_lift_rec; try omega. unfold plus. 
+repeat (unfold subst_rec; fold subst_rec; insert_Ref_out).
+unfold lift. rewrite ! lift_rec_lift_rec; try omega. unfold plus. 
 rewrite ! subst_rec_lift_rec; try omega.  
 rewrite ! lift_rec_null. 
 eapply transitive_red. eapply preserves_app_sf_red. 
-eapply fst_preserves_sf_red. eapply2 fst_out. auto. 
-eapply transitive_red. eapply preserves_app_sf_red. 
-eapply2 fst_out. auto. auto. 
+eapply2 fst_out. auto. auto.  
 Qed. 
 
 
-Lemma add_red_add: 
-forall i u sigma sigma2, 
-sf_red (App (App add sigma) (App (App (Op Aop) add) (s_op2 (s_op2 sigma2 i) u)))
-        (App (App (Op Aop) add) (s_op2 (s_op2 (App (App (App (Op Aop) add) sigma) sigma2) i) 
-        (App (App (App (Op Aop) add) sigma) u))). 
-Proof.
-intros. unfold_op;  unfold add at 1. eval_tac. 
-eapply transitive_red. eapply2 Y3_fix. 
-replace (App (App (Op Aop) (Y_k 3)) add_fn) with add by auto. 
-unfold add_fn.
-eapply transitive_red. 
-eapply preserves_app_sf_red. 
-eapply2 star_opt_beta2.  auto. 
-unfold subst; rewrite ! subst_rec_preserves_extension. 
-eapply transitive_red. eapply2 extensions_by_matchfail.
-eapply2 matchfail_compound_l. eapply2 matchfail_compound_r. 
-eapply2 matchfail_compound_l. eapply2 matchfail_compound_r. 
-eapply2 matchfail_compound_l. unfold A_k; auto. eapply2 matchfail_compound_r. 
-unfold_op; auto. 
-eapply2 matchfail_compound_l. unfold A_k; auto. eapply2 matchfail_compound_l. 
-unfold_op; eapply2 matchfail_op. unfold factorable. left; eauto. discriminate. 
-(* 1 *) 
-eapply transitive_red. eapply2 extensions_by_matchfail.
-eapply2 matchfail_compound_l. eapply2 matchfail_compound_r. 
-eapply2 matchfail_compound_r. eapply2 program_matching. 
-unfold program; auto.
-(* 2 *)  
-unfold add_fn. 
-unfold extension at 1. 
-rewrite star_opt_occurs_true. 2: cbv; auto.  2: discriminate. 
-rewrite (star_opt_occurs_true s_op). 2: cbv; auto. 2: discriminate.  
-rewrite star_opt_occurs_true. 2: cbv; auto. 
-2: rewrite star_opt_occurs_true. 2: discriminate. 2: cbv; auto. 
-2: discriminate. 
-unfold var_fn,tag at 1. 
-rewrite star_opt_eta. 2: cbv; auto.  
-unfold subst, subst_rec; fold subst_rec. insert_Ref_out. 
-rewrite subst_rec_closed; [|auto]. unfold pred. 
-rewrite star_opt_occurs_true. 2: cbv; auto. 2: discriminate. 
-rewrite (star_opt_occurs_true  (App (Op Sop) _)). 
-2: cbv; auto. 2: discriminate. 
-(* 2 *) 
-eapply2 matchfail_compound_l. eapply2 matchfail_compound_r. 
-unfold star_opt at 2 1. unfold occurs0; fold occurs0. 
-rewrite orb_false_l. 
-rewrite star_opt_occurs_true. 2: cbv; auto. 2: discriminate. 
-eapply2 matchfail_compound_l. eapply2 matchfail_op. 
-unfold factorable. right; auto. discriminate. 
-(* 1 *) 
-eapply transitive_red. eapply2 extensions_by_matchfail.
-eapply2 matchfail_compound_l. eapply2 matchfail_compound_r. 
-eapply2 matchfail_compound_l. eapply2 matchfail_compound_r. 
-eapply2 matchfail_compound_l. eapply2 matchfail_compound_r. 
-unfold_op; auto. 
-eapply2 matchfail_compound_l. eapply2 matchfail_compound_l. 
-eapply2 matchfail_op. 
-unfold factorable. unfold_op; left; eauto. discriminate. 
-(* 1 *) 
-eapply transitive_red. eapply2 extensions_by_matching. 
-eapply2 match_app. eapply2 match_app. eapply2 match_app. 
-unfold map, app, length, fold_left, subst. 
-unfold pattern_size; fold pattern_size. unfold plus; fold plus. 
-unfold_op.
-rewrite ! subst_rec_app at 1. rewrite ! subst_rec_op at 1. 
-repeat (rewrite subst_rec_ref at 1; insert_Ref_out). unfold lift. 
-rewrite ! lift_rec_lift_rec; try omega. unfold plus. 
-rewrite ! subst_rec_lift_rec; try omega.
-rewrite ! lift_rec_null.
-auto. 
-Qed.
-
-
-Lemma add_red_var_unequal: 
-forall i u sigma j, program i -> program j -> i <> j -> 
-sf_red (App (App add (s_op2 (s_op2 sigma i) u)) (var j)) (App sigma (var j)).       
-Proof.
-intros. unfold_op;  unfold add at 1. eval_tac. 
-eapply transitive_red. eapply2 Y3_fix. 
-replace (App (App (Op Aop) (Y_k 3)) add_fn) with add by auto. 
-unfold add_fn.
-eapply transitive_red. 
-eapply preserves_app_sf_red. 
-eapply2 star_opt_beta2.  auto. 
-unfold subst; rewrite ! subst_rec_preserves_extension. 
-eapply transitive_red. eapply2 extensions_by_matchfail.
-eapply2 matchfail_compound_l. eapply2 matchfail_compound_r. 
-eapply2 matchfail_compound_l. eapply2 matchfail_compound_r. 
-eapply2 matchfail_compound_l. unfold A_k; auto. eapply2 matchfail_compound_r. 
-unfold_op; auto. 
-eapply2 matchfail_compound_l. unfold A_k; auto. eapply2 matchfail_compound_l. 
-unfold_op; eapply2 matchfail_op. unfold factorable. left; eauto. discriminate. 
-eapply transitive_red. eapply2 extensions_by_matching.
-eapply2 match_app. eapply2 match_app. eapply2 match_app. 
-eapply2 program_matching. 
-unfold program; auto.
-eapply2 program_matching.  unfold program; auto. 
-unfold map, app, length, fold_left, subst. 
-unfold pattern_size; fold pattern_size.
-rewrite ! pattern_size_closed; auto.  unfold plus; fold plus. 
-unfold_op.
-rewrite ! subst_rec_app. rewrite ! subst_rec_op at 1. 
-rewrite ! subst_rec_preserves_snd_projection. 
-rewrite ! subst_rec_preserves_fst_projection. 
-repeat (rewrite subst_rec_ref at 1; insert_Ref_out). unfold lift. 
-rewrite ! lift_rec_lift_rec; try omega. unfold plus. 
-rewrite ! subst_rec_lift_rec; try omega.
-rewrite ! lift_rec_null.
-auto. 
-eapply transitive_red. eapply preserves_app_sf_red. eapply preserves_app_sf_red. 
-eapply preserves_app_sf_red. auto. 
-eapply transitive_red. eapply snd_preserves_sf_red. eapply2 fst_out.
-eapply2 snd_out.  
-eapply transitive_red. eapply snd_out. auto. 
-eapply preserves_app_sf_red.
-eapply fst_preserves_sf_red. eapply2 fst_out. auto. 
-eapply transitive_red. eapply preserves_app_sf_red. eapply preserves_app_sf_red.
-eapply2 unequal_programs. auto. auto. eval_tac. 
-eapply transitive_red. eapply preserves_app_sf_red. eapply2 fst_out. auto. 
-auto. 
-Qed.
-
-Lemma add_red_var_equal: 
-forall i u sigma, program i -> 
-sf_red (App (App add (s_op2 (s_op2 sigma i) u)) (var i)) u.       
-Proof.
-intros. unfold_op;  unfold add at 1. eval_tac. 
-eapply transitive_red. eapply2 Y3_fix. 
-replace (App (App (Op Aop) (Y_k 3)) add_fn) with add by auto. 
-unfold add_fn.
-eapply transitive_red. 
-eapply preserves_app_sf_red. 
-eapply2 star_opt_beta2.  auto. 
-unfold subst; rewrite ! subst_rec_preserves_extension. 
-eapply transitive_red. eapply2 extensions_by_matchfail.
-eapply2 matchfail_compound_l. eapply2 matchfail_compound_r. 
-eapply2 matchfail_compound_l. eapply2 matchfail_compound_r. 
-eapply2 matchfail_compound_l. unfold A_k; auto. eapply2 matchfail_compound_r. 
-unfold_op; auto. 
-eapply2 matchfail_compound_l. unfold A_k; auto. eapply2 matchfail_compound_l. 
-unfold_op; eapply2 matchfail_op. unfold factorable. left; eauto. discriminate. 
-eapply transitive_red. eapply2 extensions_by_matching.
-eapply2 match_app. 
-eapply2 program_matching. 
-unfold program; auto. 
-unfold map, app, length, fold_left, subst. 
-unfold pattern_size; fold pattern_size.
-rewrite ! pattern_size_closed; auto.  unfold plus; fold plus. 
-unfold_op.
-rewrite ! subst_rec_app. rewrite ! subst_rec_op at 1. 
-rewrite ! subst_rec_preserves_snd_projection. 
-rewrite ! subst_rec_preserves_fst_projection. 
-repeat (rewrite subst_rec_ref at 1; insert_Ref_out). unfold lift. 
-rewrite ! lift_rec_lift_rec; try omega. unfold plus. 
-rewrite ! subst_rec_lift_rec; try omega.
-rewrite ! lift_rec_null.
-auto. 
-eapply transitive_red. eapply preserves_app_sf_red. eapply preserves_app_sf_red. 
-eapply preserves_app_sf_red. auto. 
-eapply transitive_red. eapply snd_preserves_sf_red. eapply2 fst_out.
-eapply2 snd_out.  eapply2 snd_out. 
-eapply transitive_red. eapply preserves_app_sf_red. 
-eapply transitive_red. eapply fst_preserves_sf_red. eapply2 fst_out.
-eapply2 fst_out. auto. auto. 
-eapply transitive_red. eapply preserves_app_sf_red. eapply preserves_app_sf_red.
-eapply2 equal_programs. auto. auto. eval_tac. 
-Qed.
-
-
-
-Lemma add_red_tag: 
-forall sigma M N, sf_red (App (App add sigma) (tag M N)) 
-                         (App (App (App (App (Op Aop) add) sigma) M) 
-                         (App (App (App (Op Aop) add) sigma) N)). 
-Proof.
-intros. unfold add at 1. eval_tac. 
-eapply transitive_red. eapply2 Y3_fix. 
-replace (App (App (Op Aop) (Y_k 3)) add_fn) with add by auto. 
-unfold add_fn.
-eapply transitive_red. 
-eapply preserves_app_sf_red. 
-eapply2 star_opt_beta2.  auto. 
-unfold subst; rewrite ! subst_rec_preserves_extension. 
-eapply transitive_red. eapply2 extensions_by_matching.
-eapply2 match_app. eapply2 match_app. 
-eapply2 match_app. eapply2 match_app. 
-eapply2 match_app. eapply2 program_matching. 
-unfold program; auto. 
-unfold map, app, length, fold_left, subst. 
-unfold pattern_size; fold pattern_size.
-rewrite ! pattern_size_closed; auto.  unfold plus; fold plus. 
-unfold_op.
-repeat (unfold subst_rec; fold subst_rec; insert_Ref_out; unfold pred). 
-unfold lift. rewrite ! lift_rec_lift_rec; try omega. unfold plus. 
-rewrite ! subst_rec_lift_rec; try omega.
-rewrite ! lift_rec_null.
-auto. 
-Qed. 
-  
-
-Lemma add_red_abs : 
-forall xs sigma x t sigma2, 
-  sf_red (App (App add sigma2) (abs xs (s_op2 sigma x) t))
-         (abs xs (s_op2 (App (App (App (Op Aop) add) sigma2) sigma) x) t)
-.
-Proof.
-intros; unfold add; unfold abs at 1. 
-eval_tac. 
-eapply transitive_red. eapply2 Y3_fix. 
-unfold add_fn at 1. 
-eapply  transitive_red. eapply preserves_app_sf_red.  
-eapply star_opt_beta2. auto.
-unfold subst. rewrite ! subst_rec_preserves_extension. 
-eapply  transitive_red. eapply2 extensions_by_matchfail. 
-eapply2 matchfail_compound_l. 
-eapply2 matchfail_compound_r. 
-eapply2 matchfail_compound_l. 
-eapply2 matchfail_compound_r. 
-eapply2 matchfail_compound_l. 
-eapply2 matchfail_compound_r. 
-eapply2 matchfail_compound_l. 
-eapply2 matchfail_compound_r. 
-unfold_op; eapply match_op.
-eapply2 matchfail_compound_l. 
-eapply2 matchfail_compound_l. 
-eapply2 matchfail_op. unfold_op; 
-unfold factorable; split_all; left; eauto. discriminate. 
-eapply  transitive_red. 
-eapply2 extensions_by_matchfail.
-eapply2 matchfail_compound_l. 
-eapply2 matchfail_compound_r. 
-eapply2 matchfail_compound_l. 
-eapply2 matchfail_compound_r. 
-eapply2 matchfail_compound_l. 
-eapply2 matchfail_compound_r.
-unfold_op; eapply match_op.
-eapply2 matchfail_compound_l. 
-eapply2 matchfail_compound_l. 
-eapply matchfail_op. unfold factorable; split_all; eauto. discriminate.
-eapply  transitive_red. eapply2 extensions_by_matching. 
-unfold_op. 
-eapply2 match_app. 
-eapply2 match_app. 
-eapply2 match_app. 
-eapply2 match_app.
-eapply2 match_app. 
-eapply2 match_app.
-unfold map, app, length, fold_left. 
-unfold_op; unfold pattern_size; fold pattern_size; unfold plus; fold plus.
-unfold subst; rewrite ! subst_rec_app. rewrite ! subst_rec_op. 
-unfold lift; rewrite ! lift_rec_null. 
-do 20 (rewrite subst_rec_ref at 1; insert_Ref_out; unfold pred). 
-do 10 (rewrite subst_rec_ref at 1; insert_Ref_out; unfold pred). 
-unfold lift; rewrite ! lift_rec_lift_rec; try omega. unfold plus. 
-rewrite ! subst_rec_lift_rec; try omega.  rewrite ! lift_rec_null.
-insert_Ref_out. 
-repeat (unfold subst_rec; fold subst_rec; insert_Ref_out). 
-unfold lift; rewrite ! lift_rec_lift_rec; try omega. unfold plus. 
-rewrite ! subst_rec_lift_rec; try omega.  rewrite ! lift_rec_null.
-auto. 
-Qed. 
-
-
-(* 
-abs (A y ys) sigma_x t u  --> abs ys (S(S sigma_x u) y) t
-abs nil sigma_x t u --> act t (S sigma_x u) 
-act y sigma --> applysub sigma y 
-applysub (S (S sigma x) u) x -> u 
-applysub (S (S sigma x) u) y -> applysub sigma y 
-applysub nil x ---> x 
-*) 
 
