SF_calculus/Adding.v
@@ -22,8 +22,9 @@
 (*                                                                    *)
 (**********************************************************************)
 
-
-
+(* 
+Add LoadPath ".." as IntensionalLib.
+*) 
 Require Import Arith Omega Max Bool List.
 Require Import IntensionalLib.SF_calculus.General.  
 Require Import IntensionalLib.SF_calculus.SF_Terms.  
@@ -130,56 +131,91 @@ add sigma i traverses sigma, looking for i.
 
 *) 
 
-Definition add_fn := star_opt (star_opt (* recursion argument and sigma *) 
+Definition swap M N := App
+  (App (Op Sop)
+     (App
+        (App (Op Sop)
+           (App (App (Op Sop) (App (App (Op Fop) (Op Fop)) (Op Sop)))
+              (App (App (Op Sop) (App (App (Op Fop) (Op Fop)) (App (Op Sop) (App (App (Op Fop) (Op Fop)) M))))
+                 (App (Op Fop) (Op Fop)))))
+        (App (App (Op Fop) (Op Fop)) (App (App (Op Sop) (App (Op Fop) (Op Fop))) (App (Op Fop) (Op Fop))))))
+  (App (App (Op Fop) (Op Fop)) N)
+.
+
+Lemma swap_val: forall M N, swap M N = 
+App (App (Op Sop) (star_opt (app_comb (lift 1 M) (Ref 0)))) (App (App (Op Fop) (Op Fop)) N).
+Proof.
+intros; unfold swap, app_comb; unfold_op. 
+rewrite star_opt_occurs_true. 
+2: unfold occurs0; fold occurs0. 2: rewrite ! orb_true_r. 2: cbv; auto.
+2: discriminate. 
+rewrite star_opt_occurs_true. 
+2: unfold occurs0; fold occurs0. 2: rewrite ! orb_true_r. 2: cbv; auto.
+2: discriminate. 
+rewrite star_opt_occurs_true. 
+2: unfold occurs0; fold occurs0. 2: rewrite ! orb_true_r. 2: cbv; auto.
+2: discriminate. 
+ rewrite star_opt_eta. 2: auto. 
+unfold star_opt at 1.
+ rewrite star_opt_occurs_false. 
+2: simpl; unfold lift; rewrite occurs_lift_rec_zero; auto.
+unfold_op; unfold lift, subst, subst_rec; fold subst_rec.
+rewrite subst_rec_lift_rec; try omega. 
+rewrite lift_rec_null.  
+rewrite star_opt_closed; auto. 
+Qed.
+
+Lemma subst_rec_preserves_swap: 
+forall M N P k, subst_rec (swap M N) P k = swap (subst_rec M P k) (subst_rec N P k).
+Proof. intros; unfold swap, subst_rec; auto. Qed. 
+
+Lemma pattern_size_swap: 
+forall M N, pattern_size(swap M N) = pattern_size M + pattern_size N. 
+Proof. intros; unfold swap, pattern_size; fold pattern_size; omega.  Qed. 
+
+Lemma pattern_size_app_comb: 
+forall M N, pattern_size(app_comb M N) = pattern_size M + pattern_size N. 
+Proof. intros; unfold app_comb. unfold_op; unfold  pattern_size; fold pattern_size; omega.  Qed. 
+
+
+Definition add_fn := star_opt (star_opt (star_opt 
+(* recursion argument, (sigma,x) u  *) 
 (* tag *) 
-(extension (app_comb(app_comb(app_comb (Y_k 3) (Ref 2)) 
-(Ref 1)) (Ref 0)) 
-           (App (App (app_comb(Ref 4) (Ref 3)) (Ref 1))
-                (App (app_comb(Ref 4) (Ref 3)) (Ref 0)))
+(extension (app_comb(app_comb(app_comb (Y_k 3) (Ref 2)) (Ref 1)) (Ref 0)) 
+        (App (App (app_comb (app_comb (Ref 5) (Ref 4)) (Ref 3)) (Ref 1))
+             (App (app_comb (app_comb (Ref 5) (Ref 4)) (Ref 3)) (Ref 0)))
 (* var *) 
-(extension (app_comb (app_comb(Y_k 3) var_fn) (Ref 0))
+(extension (app_comb (app_comb(Y_k 3) (Ref 1)) (Ref 0))  (* var y *) 
                      (App (App (App (App equal_comb (Ref 0)) 
-                                    (snd_projection (fst_projection (Ref 1)))) (* x *) 
-                               (snd_projection (Ref 1))) (* u *) 
-                          (App (fst_projection (fst_projection (Ref 1)))  (* sigma *) 
-                               (app_comb (app_comb(Y_k 3) var_fn) (Ref 0))))
-(* abs *)
-(extension (app_comb (app_comb 
-(app_comb (app_comb(Y_k 4) (Ref 4)) (Ref 3)) (s_op2 (Ref 2) (Ref 1)))
-(Ref 0))
-           (app_comb (app_comb (app_comb 
-(app_comb (Y_k 4) (Ref 4)) (Ref 3))
-                                         (s_op2 (App (app_comb(Ref 6) (Ref 5)) (Ref 2)) (Ref 1)))
-                               (Ref 0))
+                                     (snd_projection (Ref 3))) (* y = x *) 
+                               (Ref 2))  (* u *) 
+                          (App (fst_projection (Ref 3)) 
+                               (app_comb (app_comb(Y_k 3) (Ref 1)) (Ref 0))))
+                                          (* sigma (var y) *) 
 (* add  *) 
 (* | Add i u sigma => App (App (Op Aop) add) (s_op2 (s_op2 (lambda_to_fieska sigma) (ref i)) (lambda_to_fieska u))
 *) 
-(extension (app_comb(Ref 3) 
-                (App (App (Op Sop) (App (App (Op Sop) (Ref 2)) (Ref 1))) (Ref 0)))
-           (app_comb(Ref 3) 
-                (App (App (Op Sop) 
-                (App (App (Op Sop) (App (app_comb(Ref 5) (Ref 4)) (Ref 2))) (Ref 1)))
-                (App (app_comb(Ref 5) (Ref 4)) (Ref 0))))
-(* Nil *) 
-(fst_projection (fst_projection (Ref 0)))))))).  
+(extension (app_comb (app_comb (app_comb (Y_k 4) (Ref 2)) (Ref 1)) (Ref 0))
+  (* add (sigma2, x2) u *) 
+   (app_comb (app_comb (app_comb (Y_k 4) (Ref 2))
+     (s_op2 (App (app_comb (app_comb (Ref 5) (Ref 4)) (Ref 3)) (fst_projection (Ref 1)))
+        (snd_projection (Ref 1))))
+     (App (app_comb (app_comb (Ref 5) (Ref 4)) (Ref 3)) (Ref 0)))
+(* abs = swap (app_comb add (s_op2 sigma x)) t *) 
+(extension (swap (app_comb (Ref 3) (App (App (Op Sop) (Ref 2)) (Ref 1))) (Ref 0))
+           (swap (app_comb (Ref 3) (App (App (Op Sop) 
+                                             (App (app_comb (app_comb (Ref 6) (Ref 5)) (Ref 4)) (Ref 2))) 
+                                   (Ref 1)))
+                 (Ref 0))
+(* dummy case *) 
+(fst_projection (Ref 1))
+)))))).
 
-Definition add :=  app_comb(Y_k 3) add_fn.
+Definition add :=  app_comb(Y_k 4) add_fn.
 
 
-Definition abs_fn := star_opt  (* rec'n argument *) 
-(extension (App (App s_op (Ref 1)) (Ref 0)) (* y::ys *) 
-           (star_opt (star_opt (star_opt (* sigma_x t u *) 
-             (app_comb (app_comb (app_comb (Ref 5) (Ref 3)) 
-                                 (s_op2 (app_comb add (s_op2 (Ref 2) (Ref 0))) (Ref 4)))
-                       (Ref 1)))))
-           (App k_op (star_opt (star_opt (star_opt (App (app_comb add 
-                                                        (s_op2 (Ref 2) (Ref 0)))
-                                                        (Ref 1)))))))
-.
+Definition abs sigma x t := swap (app_comb add (s_op2 sigma x)) t .
 
-Definition abs xs sigma_x t := 
-  app_comb (app_comb (app_comb 
-  (app_comb(Y_k 4) abs_fn) xs) sigma_x) t. 
 
 
 Lemma add_closed: maxvar add = 0.
@@ -190,14 +226,285 @@ repeat (rewrite maxvar_extension; rewrite ? maxvar_app; rewrite ? maxvar_app_com
 cbv.  auto. 
 Qed. 
 
-Lemma abs_fn_closed: maxvar abs_fn = 0. 
+
+Lemma abs_red : 
+forall sigma x t u, sf_red (App (abs sigma x t) u) 
+                           (App (app_comb (app_comb add (s_op2 sigma x)) u) t). 
 Proof.
-unfold abs_fn.  rewrite ! maxvar_star_opt. 
-rewrite maxvar_extension.  rewrite ? maxvar_star_opt. rewrite ? maxvar_app_comb.
-rewrite ? maxvar_app. rewrite ! maxvar_star_opt. 
-unfold_op. unfold pattern_size. 
-rewrite ! maxvar_app. rewrite maxvar_app_comb. rewrite add_closed. cbv.  auto. 
+intros; unfold abs. 
+rewrite swap_val. 
+eapply succ_red. eapply2 s_red. 
+eapply transitive_red. eapply preserves_app_sf_red. eapply2 star_opt_beta. 
+eval_tac.
+unfold subst, lift. rewrite ! subst_rec_preserves_app_comb.
+rewrite subst_rec_lift_rec; try omega. 
+unfold subst_rec; insert_Ref_out. 
+unfold lift; rewrite ! lift_rec_null. 
+ auto. 
 Qed. 
+
+
+
+Lemma add_red_tag: 
+forall sigma_x u M N, sf_red (App (App (App add sigma_x) u) (tag M N)) 
+                         (App (App (app_comb (app_comb add sigma_x) u) M)
+                              (App (app_comb (app_comb add sigma_x) u) N)).
+Proof.
+intros. unfold add at 1. 
+eapply transitive_red. eapply preserves_app_sf_red. 
+eapply preserves_app_sf_red. eapply2 app_comb_red.
+auto. auto. 
+eapply transitive_red. eapply2 Y4_fix. 
+replace (app_comb (Y_k 4) add_fn) with add by auto. 
+unfold add_fn.
+eapply transitive_red. 
+eapply preserves_app_sf_red. 
+eapply2 star_opt_beta3.  auto. 
+unfold subst; rewrite ! subst_rec_preserves_extension. 
+eapply transitive_red. 
+ eapply2 extensions_by_matching.
+unfold tag, tag_fix.  
+unfold app_comb; unfold_op. 
+eapply2 match_app. eapply2 match_app.  
+eapply2 match_app. eapply2 match_app. 
+eapply2 match_app. eapply2 match_app. 
+eapply2 match_app. eapply2 match_app. 
+eapply2 match_app. eapply2 match_app. 
+eapply2 match_app. eapply2 match_app. 
+eapply2 match_app. eapply2 program_matching. 
+unfold program; auto. eapply2 program_matching. 
+unfold program; auto. eapply2 program_matching. 
+unfold program; auto. eapply2 program_matching. 
+unfold program; auto.
+(* 1 *)  
+unfold map, app, length, fold_left, subst.
+unfold subst_rec; fold subst_rec. 
+rewrite ! subst_rec_preserves_app_comb. 
+rewrite ! pattern_size_app_comb.   
+unfold pattern_size; fold pattern_size. 
+rewrite pattern_size_closed; auto.  unfold plus; fold plus. 
+unfold lift. rewrite ! lift_rec_lift_rec; try omega. unfold plus. 
+repeat (rewrite subst_rec_ref; insert_Ref_out; unfold pred). 
+unfold lift. rewrite ! lift_rec_lift_rec; try omega. unfold plus. 
+repeat (rewrite subst_rec_ref; insert_Ref_out; unfold pred). 
+rewrite ! subst_rec_lift_rec; try omega.
+rewrite ! lift_rec_null. auto. 
+Qed. 
+  
+
+
+Lemma add_red_var_unequal: 
+forall i u sigma j, program i -> program j -> i <> j -> 
+sf_red (App (App (App add (s_op2 sigma i)) u) (var j)) (App sigma (var j)).       
+Proof.
+intros. unfold_op;  unfold add at 1. 
+eapply transitive_red. eapply preserves_app_sf_red. 
+eapply preserves_app_sf_red. eapply2 app_comb_red. 
+auto. auto. 
+eapply transitive_red. eapply2 Y4_fix. 
+replace (app_comb (Y_k 4) add_fn) with add by auto. 
+unfold add_fn.
+eapply transitive_red. 
+eapply preserves_app_sf_red. 
+eapply2 star_opt_beta3.  auto. 
+unfold subst; rewrite ! subst_rec_preserves_extension. 
+eapply transitive_red. eapply2 extensions_by_matchfail.
+unfold var, var_fix, var_fn, app_comb; unfold_op. 
+eapply2 matchfail_compound_l. eapply2 matchfail_compound_r. 
+eapply2 matchfail_compound_l. eapply2 matchfail_compound_r.
+eapply2 matchfail_compound_r. 
+eapply2 matchfail_compound_l. eapply2 matchfail_compound_r. 
+eapply2 matchfail_compound_l. eapply2 matchfail_compound_r.
+eapply2 matchfail_compound_r. unfold Y_k, app_comb; unfold_op. 
+eapply2 matchfail_compound_l. eapply2 matchfail_compound_r. 
+eapply2 matchfail_compound_l. eapply2 matchfail_compound_r.
+eapply2 matchfail_compound_r. 
+eapply2 matchfail_compound_l. eapply2 matchfail_compound_r. 
+eapply2 matchfail_compound_l. eapply2 matchfail_compound_r.
+eapply2 matchfail_compound_r. unfold A_k, app_comb; unfold_op. 
+eapply2 matchfail_compound_l. eapply2 matchfail_compound_r. 
+eapply2 matchfail_compound_l. eapply2 matchfail_compound_l.
+eapply2 matchfail_op. unfold factorable. left; eauto. discriminate.
+(* 1 *)  
+eapply transitive_red. eapply2 extensions_by_matching.
+unfold var, var_fix, app_comb; unfold_op. 
+eapply2 match_app. eapply2 match_app. eapply2 match_app. 
+eapply2 match_app. eapply2 match_app. eapply2 match_app. 
+eapply2 match_app. eapply2 match_app. 
+apply program_matching. 
+unfold program; split. 
+nf_out.  auto. 
+apply program_matching. 
+unfold program; split. 
+nf_out.  auto. 
+apply program_matching. 
+unfold program; split. 
+nf_out.  auto. 
+(* 1 *) 
+unfold map, app, length, fold_left, subst. 
+unfold app_comb; unfold_op. 
+unfold pattern_size; fold pattern_size.
+rewrite ! pattern_size_closed; auto.  unfold plus; fold plus. 
+rewrite ! subst_rec_app. rewrite ! (subst_rec_closed equal_comb). 2: auto. 
+rewrite ! subst_rec_preserves_snd_projection. 
+rewrite ! subst_rec_preserves_fst_projection. 
+unfold lift. rewrite ! lift_rec_null.
+repeat (rewrite subst_rec_ref at 1; insert_Ref_out). 
+unfold lift; rewrite ! lift_rec_lift_rec; try omega. unfold plus. 
+rewrite ! subst_rec_lift_rec; try omega.
+rewrite ! lift_rec_null.
+unfold subst_rec; fold subst_rec. 
+rewrite ! (subst_rec_closed (Y_k _)); try (rewrite Y_k_closed; omega). 
+eapply transitive_red. eapply preserves_app_sf_red. eapply preserves_app_sf_red. 
+eapply preserves_app_sf_red. auto. 
+eapply2 snd_out. auto.   
+eapply transitive_red. eapply preserves_app_sf_red. eapply2 fst_out. auto. auto. 
+eapply transitive_red. eapply preserves_app_sf_red. eapply preserves_app_sf_red.
+eapply2 unequal_programs. auto. auto. 
+eval_tac. eval_tac. 
+Qed.
+
+Lemma add_red_var_equal: 
+forall i u sigma, program i -> 
+sf_red (App (App (App add (s_op2 sigma i)) u) (var i)) u.       
+Proof.
+intros. unfold_op;  unfold add at 1. 
+eapply transitive_red. eapply preserves_app_sf_red.  
+eapply preserves_app_sf_red. eapply2 app_comb_red. 
+auto. auto. 
+eapply transitive_red. eapply2 Y4_fix. 
+replace (app_comb (Y_k 4) add_fn) with add by auto. 
+unfold add_fn.
+eapply transitive_red. 
+eapply preserves_app_sf_red. 
+eapply2 star_opt_beta3.  auto. 
+unfold subst; rewrite ! subst_rec_preserves_extension. 
+eapply transitive_red. eapply2 extensions_by_matchfail.
+unfold var, var_fix, var_fn, app_comb; unfold_op. 
+eapply2 matchfail_compound_l. eapply2 matchfail_compound_r. 
+eapply2 matchfail_compound_l. eapply2 matchfail_compound_r.
+eapply2 matchfail_compound_r. 
+eapply2 matchfail_compound_l. eapply2 matchfail_compound_r. 
+eapply2 matchfail_compound_l. eapply2 matchfail_compound_r.
+eapply2 matchfail_compound_r. unfold Y_k, app_comb; unfold_op. 
+eapply2 matchfail_compound_l. eapply2 matchfail_compound_r. 
+eapply2 matchfail_compound_l. eapply2 matchfail_compound_r.
+eapply2 matchfail_compound_r. 
+eapply2 matchfail_compound_l. eapply2 matchfail_compound_r. 
+eapply2 matchfail_compound_l. eapply2 matchfail_compound_r.
+eapply2 matchfail_compound_r. unfold A_k, app_comb; unfold_op. 
+eapply2 matchfail_compound_l. eapply2 matchfail_compound_r. 
+eapply2 matchfail_compound_l. eapply2 matchfail_compound_l.
+eapply2 matchfail_op. unfold factorable. left; eauto. discriminate.
+(* 1 *)  
+eapply transitive_red. eapply2 extensions_by_matching.
+unfold var, var_fix, app_comb; unfold_op. 
+eapply2 match_app. eapply2 match_app. eapply2 match_app. 
+eapply2 match_app. eapply2 match_app. eapply2 match_app. 
+eapply2 match_app. eapply2 match_app. 
+eapply2 program_matching. 
+unfold program; split. nf_out. cbv; auto. 
+eapply2 program_matching. 
+unfold program; split. nf_out. cbv; auto. 
+eapply2 program_matching. 
+unfold program; split. nf_out. cbv; auto. 
+unfold map, app, length, fold_left, subst. 
+unfold app_comb at 3 4 5 6 7 8; unfold_op. 
+unfold pattern_size; fold pattern_size.
+rewrite ! pattern_size_closed; auto.  unfold plus; fold plus. 
+rewrite ! subst_rec_app. rewrite ! (subst_rec_closed equal_comb) at 1. 2: auto. 
+2: auto. 2: auto. 2: auto. 2: auto. 
+rewrite ! subst_rec_preserves_snd_projection. 
+rewrite ! subst_rec_preserves_fst_projection. 
+repeat (rewrite subst_rec_ref at 1; insert_Ref_out). unfold lift. 
+rewrite ! lift_rec_lift_rec; try omega. unfold plus. 
+rewrite ! subst_rec_lift_rec; try omega.
+rewrite ! lift_rec_null.
+eapply transitive_red. eapply preserves_app_sf_red. eapply preserves_app_sf_red. 
+eapply preserves_app_sf_red. auto. eapply2 snd_out. auto. auto. 
+(* 1 *) 
+eapply transitive_red. eapply preserves_app_sf_red. eapply preserves_app_sf_red.
+eapply2 equal_programs. auto. auto. 
+eval_tac.  
+Qed.
+
+
+
+Lemma add_red_abs : 
+forall sigma x t sigma_y u, 
+  sf_red (App (App (App add sigma_y) u) (abs sigma x t))
+         (abs (App (app_comb (app_comb add sigma_y) u) sigma) x t). 
+Proof.
+intros. unfold add at 1. 
+eapply transitive_red. eapply preserves_app_sf_red. 
+eapply preserves_app_sf_red. eapply2 app_comb_red. 
+auto. auto. 
+eapply transitive_red. eapply2 Y4_fix. 
+replace (app_comb (Y_k 4) add_fn) with add by auto. 
+unfold add_fn.
+eapply transitive_red. 
+eapply preserves_app_sf_red. 
+eapply2 star_opt_beta3.  auto. 
+unfold subst; rewrite ! subst_rec_preserves_extension. 
+eapply transitive_red. eapply2 extensions_by_matchfail.
+unfold abs, swap, app_comb; unfold_op; auto. 
+eapply2 matchfail_compound_l. 
+eapply2 matchfail_compound_r. 
+eapply2 matchfail_compound_l. 
+eapply2 matchfail_compound_r. 
+eapply2 matchfail_compound_l. 
+eapply2 matchfail_compound_l. 
+eapply2 matchfail_op. 
+unfold factorable; eauto. discriminate. 
+(* 1 *) 
+eapply  transitive_red. 
+eapply2 extensions_by_matchfail.
+unfold abs, swap, app_comb; unfold_op; auto. 
+eapply2 matchfail_compound_l. 
+eapply2 matchfail_compound_r. 
+eapply2 matchfail_compound_l. 
+eapply2 matchfail_compound_r. 
+eapply2 matchfail_compound_l. 
+eapply2 matchfail_compound_l. 
+eapply2 matchfail_op. 
+unfold factorable; eauto. discriminate. 
+(* 1 *) 
+eapply  transitive_red. 
+eapply2 extensions_by_matchfail.
+unfold abs, swap, app_comb; unfold_op; auto. 
+eapply2 matchfail_compound_l. 
+eapply2 matchfail_compound_r. 
+eapply2 matchfail_compound_l. 
+eapply2 matchfail_compound_r. 
+eapply2 matchfail_compound_l. 
+eapply2 matchfail_compound_l. 
+eapply2 matchfail_op. 
+unfold factorable; eauto. discriminate. 
+(* 1 *) 
+eapply  transitive_red. 
+eapply2 extensions_by_matching.
+unfold abs, swap, app_comb; unfold_op; auto. 
+do 20 eapply2 match_app. 
+unfold map, app, length, fold_left, subst.  
+(* 1 *) 
+ unfold abs. rewrite ! subst_rec_preserves_swap. 
+rewrite ! subst_rec_preserves_app_comb. 
+rewrite ! pattern_size_swap. 
+rewrite ! pattern_size_app_comb. 
+unfold pattern_size; fold pattern_size. 
+unfold lift; rewrite ! lift_rec_null. unfold plus. 
+rewrite ! lift_rec_lift_rec; try omega. unfold plus; fold plus. 
+repeat (unfold subst_rec; fold subst_rec; insert_Ref_out). 
+rewrite ! subst_rec_preserves_app_comb. 
+repeat (unfold subst_rec; fold subst_rec; insert_Ref_out). 
+unfold lift; rewrite ! lift_rec_null. 
+rewrite ! lift_rec_lift_rec; try omega. unfold plus. 
+rewrite ! subst_rec_lift_rec; try omega. 
+rewrite ! lift_rec_null. 
+auto. 
+Qed.   
+
+
 
 
 
@@ -219,596 +526,128 @@ Ltac nf_out :=
 Lemma add_fn_normal: normal add_fn. 
 Proof. 
 eapply2 pattern_normal_zero. 
-unfold add_fn. replace 0 with (pred (pred 2)) by omega. 
+unfold add_fn. replace 0 with (pred (pred (pred 3))) by omega. 
 repeat apply pattern_normal_star_opt. unfold pred.
 apply extension_pattern_normal. 
-eapply2 pnf_break. 3: cbv; auto. 
-eapply2 pnf_break. 3: cbv; auto. 
+eapply2 pnf_break. 3: cbv; omega. 
+eapply2 pnf_break. 3: cbv; omega.  3: cbv; omega. 
 apply pattern_normal_app_comb. 
-eapply2 pnf_normal. eapply2 pnf_normal. eapply2 pnf_normal. 
-cbv; auto. 
-eapply2 pnf_break. 3: cbv; auto. 
-apply pattern_normal_app_comb. eapply2 pnf_normal. eapply2 pnf_normal. 
+apply pattern_normal_app_comb. 
+eapply2 pnf_normal.
+eapply2 pnf_normal.
+eapply2 pnf_normal.
+eapply2 pnf_normal.
+eapply2 pnf_break. 3: cbv; omega. 
+apply pattern_normal_app_comb. 
+apply pattern_normal_app_comb. 
+eapply2 pnf_normal.
+eapply2 pnf_normal.
+eapply2 pnf_normal.
 eapply2 pnf_normal.
 (* 1 *) 
 apply extension_pattern_normal. 
-eapply2 pnf_break. 3: cbv; auto. 
-eapply2 pnf_break. 3: cbv; auto. 
-eapply2 pnf_break. 3: cbv; auto. 
+eapply2 pnf_break. 3: cbv; auto. 3: cbv; auto. 
+eapply2 pnf_break. 3: cbv; auto. 3: cbv; auto. 
+eapply2 pnf_break. 3: cbv; auto. 3: cbv; auto. 
 eapply2 pnf_break. 
 eapply2 pnf_normal. eapply2 equal_comb_normal. 
+eapply2 pnf_normal. cbv; omega. 
 eapply2 pnf_normal.
-unfold fst_projection, snd_projection, left_projection, right_projection. 
-unfold_op. 
-eapply2 pnf_active.
-eapply2 pnf_compound. eapply2 pnf_compound.  eapply2 pnf_normal. 
-eapply2 pnf_active.
-eapply2 pnf_compound. eapply2 pnf_compound.  eapply2 pnf_normal. 
-eapply2 pnf_active.
-eapply2 pnf_compound. eapply2 pnf_compound.  eapply2 pnf_normal. 
- eapply2 pnf_normal.  eapply2 pnf_normal.  eapply2 pnf_normal. 
-eapply2 pnf_active.
-eapply2 pnf_compound. eapply2 pnf_compound.  eapply2 pnf_normal. 
- eapply2 pnf_normal.  eapply2 pnf_normal.  eapply2 pnf_normal. 
-eapply2 pnf_compound.
-eapply2 pnf_normal.   eapply2 pnf_normal.
-eapply2 pnf_active.
-eapply2 pnf_compound. eapply2 pnf_compound.  eapply2 pnf_normal. 
-eapply2 pnf_active.
-eapply2 pnf_compound. eapply2 pnf_compound.  eapply2 pnf_normal. 
- eapply2 pnf_normal.  eapply2 pnf_normal.  eapply2 pnf_normal. 
-eapply2 pnf_active.
-eapply2 pnf_compound. eapply2 pnf_compound.  eapply2 pnf_normal. 
- eapply2 pnf_normal.  eapply2 pnf_normal.  eapply2 pnf_normal. 
- eapply2 pnf_normal. nf_out.   eapply2 pnf_normal. nf_out. 
-unfold fst_projection, snd_projection, left_projection, right_projection. 
-unfold_op. 
-eapply2 pnf_active.
-eapply2 pnf_normal.   eapply2 pnf_normal. nf_out.  
-unfold fst_projection, snd_projection, left_projection, right_projection. 
-unfold_op. 
-eapply2 pnf_active. eapply2 pnf_active.
-eapply2 pnf_normal. nf_out.  eapply2 nf_active. nf_out. 
-eapply2 nf_active. nf_out. eapply2 nf_active. nf_out. 
-eapply2 nf_active. nf_out. eapply2 nf_active. nf_out.
-eapply2 nf_active. nf_out. eapply2 nf_active. nf_out.
-eapply2 nf_active. nf_out. eapply2 nf_active. nf_out.
-eapply2 nf_active. nf_out. eapply2 nf_active. nf_out.
-eapply2 nf_active. nf_out. eapply2 nf_active. nf_out.
-eapply2 nf_active. nf_out. nf_out.
-(* 3 *) 
-eapply2 pnf_normal. nf_out.  
-apply pnf_normal. apply app_comb_normal. apply app_comb_normal. 
-auto. auto. auto. 
+unfold snd_projection, right_projection.
+eapply2 nf_active. unfold_op; nf_out. 
+eapply2 pnf_normal.
+unfold fst_projection, right_projection, left_projection.
+apply pnf_normal.
+ apply nf_active. apply nf_active. nf_out. 
+apply nf_active. nf_out.  auto. auto. auto. 
+cbv; auto. 
+eapply2 nf_active. 
+nf_out. 
+cbv; auto. 
+eapply2 app_comb_normal. 
+eapply2 app_comb_normal.
+cbv; auto.  
 (* 1 *) 
 apply extension_pattern_normal.
 apply pattern_normal_app_comb. 
 apply pattern_normal_app_comb. 
-apply pnf_normal. apply app_comb_normal. apply app_comb_normal. 
-auto. auto. auto.
-unfold_op. apply pnf_compound.  apply pnf_compound.   eapply2 pnf_normal. 
-apply pnf_break. 3: simpl; omega. 
-apply pnf_normal. eapply2 app_comb_normal. eapply2 pnf_normal.
-cbv; auto. auto. eapply2 pnf_normal. auto. eapply2 pnf_normal. 
+apply pattern_normal_app_comb. 
+eapply2 pnf_normal.
+eapply2 pnf_normal. 
+unfold_op.  
+apply pnf_break. 3: cbv; omega. 3: cbv; omega. 
+apply pnf_break. 3: cbv; omega. 3: cbv; omega. 
+eapply2 pnf_normal. 
+apply pnf_break. 3: cbv; omega. 3: cbv; omega. 
+eapply2 pnf_normal. 
+repeat eapply2 app_comb_normal.
+unfold fst_projection, right_projection, left_projection. 
+apply pnf_normal. 
+apply nf_active. nf_out. 
+apply nf_active. nf_out. auto. auto. auto. auto. 
+eapply2 nf_active. 
+unfold_op; auto. 
+cbv; auto. 
+unfold snd_projection, right_projection, left_projection.
+apply pnf_normal.
+eapply2 nf_active. unfold_op; auto.
+eapply2 pnf_break. 
+eapply2 pnf_normal.
+nf_out; auto. 
+eapply2 pnf_normal.
+cbv; omega. 
 (* 1 *) 
 apply extension_pattern_normal.
-apply pattern_normal_app_comb. eapply2 pnf_normal. 
-eapply2 pnf_compound. eapply2 pnf_compound. eapply2 pnf_normal.
-eapply2 pnf_compound. eapply2 pnf_compound. eapply2 pnf_normal.
-apply pnf_break. apply pnf_normal.  nf_out. auto. auto. 
-eapply2 pnf_normal. simpl; omega. simpl; omega. eapply2 pnf_normal. 
-eapply2 pnf_break. eapply2 pnf_normal.  unfold app_comb; nf_out.
-auto. auto. eapply2 pnf_normal. simpl; omega. 
-apply pnf_normal. cbv; nf_out. 
-apply nf_active. nf_out. apply nf_active. nf_out. 
-apply nf_active. nf_out. apply nf_active. nf_out. auto. auto. nf_out. 
-auto. 
-apply nf_active; nf_out; auto. nf_out.  auto.
-apply nf_active; nf_out; auto. nf_out.  auto.
-apply nf_active; nf_out; auto.
-apply nf_active; nf_out; auto. 
-apply nf_active; nf_out; auto. nf_out. auto. 
+2: apply pnf_normal; unfold fst_projection, left_projection, right_projection.
+2: apply nf_active; nf_out; auto.
+rewrite pattern_size_swap.    
+rewrite swap_val. 
+eapply2 pnf_break. 3: cbv; omega. 
+2: eapply2 pnf_normal.
+eapply2 pnf_break. 3: cbv; omega. 
+eapply2 pnf_normal.
+rewrite pattern_size_app_comb. unfold pattern_size; fold pattern_size. 
+unfold plus; fold plus.
+cbv.  
+repeat (apply pnf_compound;[| | auto; fail]);
+try (eapply2 pnf_normal; fail). 
+eapply2 pnf_break. 
+2: eapply2 pnf_normal.  
+2: cbv;  omega. 
+apply pnf_normal; nf_out; auto. 
 Qed. 
+ 
+
+
   
 Lemma add_normal: normal add. 
 Proof. 
 unfold add. apply app_comb_normal. auto. apply add_fn_normal. 
 Qed. 
 
-Lemma abs_fn_normal: normal abs_fn. 
+Lemma abs_normal: 
+forall sigma x t, normal sigma -> normal x -> normal t -> normal (abs sigma x t).  
 Proof. 
-eapply2 pattern_normal_zero. 
-unfold abs_fn. replace 0 with (pred 1) by omega. 
-apply pattern_normal_star_opt. unfold pred.
-apply extension_pattern_normal.
-unfold_op; unfold pattern_size.   unfold plus. 
-replace 3 with (pred (pred (pred 6))) by auto. 
-repeat apply pattern_normal_star_opt. unfold pred.
-eapply2 pnf_normal.
-repeat apply app_comb_normal; auto. nf_out. 
-unfold add.  apply app_comb_normal.  auto. eapply2  add_fn_normal. 
-auto. auto. auto. 
-apply pnf_normal. unfold_op. 
-rewrite star_opt_occurs_true. 
-2: unfold app_comb; rewrite ! occurs_app. 
-2: replace (occurs0 (Ref 0)) with true by auto.  
-2: rewrite (orb_true_r (occurs0 (Op Sop) || occurs0 (Ref 2))).
-2: rewrite (orb_true_r (occurs0 k_op)).
-2: rewrite ! orb_true_r at 1. 2: rewrite ! orb_true_l at 1; auto. 
-2: discriminate.  
-apply nf_compound. nf_out. 
-repeat apply star_opt_normal. 
-apply nf_compound. apply nf_compound. nf_out. 
-repeat apply star_opt_normal.
-apply app_comb_normal. 
-apply add_normal. 
-nf_out. auto. auto. auto. cbv; auto. auto. auto. 
+intros. unfold abs, swap. nf_out. 
+eapply2 add_normal. auto. auto. auto. 
 Qed. 
-
- 
-
-Delimit Scope bigN_scope with bigN.
-Local Open Scope bigN_scope.
-
-
-Fixpoint size M := 
-match M with 
-| Ref _ => 2 
-| Op _ => 1
-| App M1 M2 => (size M2) + (size M1)
-end .
-
-
-Lemma size_var_fn : size var_fn = 1079. 
-Proof. cbv; auto. Qed. 
-
-Lemma size_add: size add = 47391.
-Proof. cbv; auto. Qed. 
-
-Lemma size_abs_fn: size abs_fn = 95603. 
-Proof. cbv; auto. Qed. 
-
-
-Lemma abs_many_red : 
-forall x1 xs sigma_x t u, sf_red (App (abs (App (App s_op x1) xs) sigma_x t) u)
-                                      (abs xs (s_op2 (app_comb add (s_op2 sigma_x u)) x1) t).
-Proof.
-intros; unfold abs, abs_fn, s_op2; unfold_op. 
-eapply transitive_red. eapply2 app_comb_red. 
-eapply transitive_red. eapply preserves_app_sf_red. eapply app_comb_red. auto. 
-eapply transitive_red. eapply preserves_app_sf_red. eapply preserves_app_sf_red. 
-eapply app_comb_red. auto. auto.
-eapply transitive_red. eapply preserves_app_sf_red. eapply preserves_app_sf_red. 
-eapply preserves_app_sf_red. eapply app_comb_red. auto. auto. auto. 
-eapply transitive_red. eapply preserves_app_sf_red. eapply Y4_fix. auto.  
-eapply transitive_red. eapply preserves_app_sf_red.  eapply preserves_app_sf_red.  
-eapply preserves_app_sf_red.  eapply preserves_app_sf_red. 
-eapply2 star_opt_beta. auto. auto. auto. auto.  
-unfold subst. rewrite subst_rec_preserves_extension. 
-eapply transitive_red. eapply preserves_app_sf_red.  eapply preserves_app_sf_red. 
- eapply preserves_app_sf_red.  
-eapply extensions_by_matching. 
-eapply match_app; nf_out. auto. auto. auto.  
-unfold map, app, length, fold_left, subst.  
-do 9 (rewrite subst_rec_preserves_star_opt at 1). 
-eapply transitive_red.  eapply2 star_opt_beta3.
-unfold pattern_size; fold pattern_size. unfold plus; fold plus. 
-unfold subst; rewrite 18? subst_rec_preserves_app_comb at 1. 
-repeat (unfold subst_rec; fold subst_rec; insert_Ref_out; unfold pred). 
-unfold lift; rewrite lift_rec_lift_rec; try omega. unfold plus.
-rewrite ! subst_rec_lift_rec; try omega. rewrite ! lift_rec_null.
-rewrite ! subst_rec_preserves_app_comb. 
-rewrite 6? (subst_rec_closed add) at 1; try (rewrite add_closed; omega). 
-repeat (unfold subst_rec; fold subst_rec; insert_Ref_out; unfold pred).  
-unfold lift; rewrite lift_rec_lift_rec; try omega. unfold plus.
-rewrite ! subst_rec_lift_rec; try omega. rewrite ! lift_rec_null.
-auto. 
-Qed. 
-
-
-Lemma abs_red : 
-forall sigma_x t u, sf_red (App (abs s_op sigma_x t) u) 
-                           (App (app_comb add (s_op2 sigma_x u)) t). 
-Proof.
-intros; unfold abs, abs_fn, s_op2; unfold_op. 
-eapply transitive_red. eapply2 app_comb_red. 
-eapply transitive_red. eapply preserves_app_sf_red. eapply app_comb_red. auto. 
-eapply transitive_red. eapply preserves_app_sf_red. eapply preserves_app_sf_red. 
-eapply app_comb_red. auto. auto.
-eapply transitive_red. eapply preserves_app_sf_red. eapply preserves_app_sf_red. 
-eapply preserves_app_sf_red. eapply app_comb_red. auto. auto. auto. 
-eapply transitive_red. eapply preserves_app_sf_red. eapply Y4_fix. auto.  
-eapply transitive_red. eapply preserves_app_sf_red.  eapply preserves_app_sf_red.  
-eapply preserves_app_sf_red.  eapply preserves_app_sf_red. 
-eapply2 star_opt_beta. auto. auto. auto. auto.  
-unfold subst. rewrite subst_rec_preserves_extension. 
-eapply transitive_red. eapply preserves_app_sf_red.  eapply preserves_app_sf_red. 
- eapply preserves_app_sf_red.  
-eapply2 extensions_by_matchfail. auto. auto. auto.  
-rewrite ! subst_rec_app; rewrite ! subst_rec_op. 
-eapply transitive_red. eapply preserves_app_sf_red. eapply preserves_app_sf_red. 
-eapply preserves_app_sf_red. eapply succ_red. eapply f_op_red. 
-rewrite ! subst_rec_preserves_star_opt. auto. auto. auto. auto. auto. 
-eapply transitive_red. eapply star_opt_beta3. 
-unfold subst. (rewrite 4? subst_rec_app at 1).
-rewrite ! subst_rec_preserves_app_comb. 
-do 4 (rewrite (subst_rec_closed add) at 1; [| rewrite add_closed; omega]).  
-repeat (unfold subst_rec; fold subst_rec; insert_Ref_out;  unfold pred).
-unfold lift.  rewrite ? lift_rec_lift_rec; try omega. unfold plus; fold plus. 
-rewrite ? subst_rec_lift_rec; try omega.
-rewrite ? lift_rec_null; try omega. auto. 
-Qed. 
-
-
-
-Lemma add_red_tag: 
-forall sigma M N, sf_red (App (App add sigma) (tag M N)) 
-                         (App (App (app_comb add sigma) M) 
-                         (App (app_comb add sigma) N)). 
-Proof.
-intros. unfold_op;  unfold add at 1. 
-eapply transitive_red. eapply preserves_app_sf_red. eapply2 app_comb_red. 
-auto. 
-eapply transitive_red. eapply2 Y3_fix. 
-replace (app_comb (Y_k 3) add_fn) with add by auto. 
-unfold add_fn.
-eapply transitive_red. 
-eapply preserves_app_sf_red. 
-eapply2 star_opt_beta2.  auto. 
-unfold subst; rewrite ! subst_rec_preserves_extension. 
-eapply transitive_red. eapply2 extensions_by_matching.
-unfold tag, tag_fix.  
-unfold app_comb; unfold_op. 
-eapply2 match_app. eapply2 match_app.  
-eapply2 match_app. eapply2 match_app. 
-eapply2 match_app. eapply2 match_app. 
-eapply2 match_app. eapply2 match_app. 
-eapply2 match_app. eapply2 match_app. 
-eapply2 match_app. eapply2 match_app. 
-eapply2 match_app. eapply2 program_matching. 
-unfold program; auto. eapply2 program_matching. 
-unfold program; auto. eapply2 program_matching. 
-unfold program; auto. eapply2 program_matching. 
-unfold program; auto. 
-unfold map, app, length, fold_left, subst. 
-unfold app_comb at 3 4 5; unfold_op. 
-unfold pattern_size; fold pattern_size. 
-rewrite pattern_size_closed; auto.  unfold plus; fold plus. 
-unfold app_comb at 3 4 5; unfold_op. 
-unfold pattern_size; fold pattern_size. 
-rewrite pattern_size_closed; auto.  unfold plus; fold plus. 
-unfold lift; rewrite ! lift_rec_null.
-rewrite ! subst_rec_app. rewrite ! subst_rec_preserves_app_comb.  
-repeat (rewrite subst_rec_ref; insert_Ref_out; unfold pred). 
-unfold lift. rewrite ! lift_rec_lift_rec; try omega. unfold plus. 
-rewrite ! subst_rec_lift_rec; try omega.
-rewrite ! lift_rec_null.
-auto. 
-Qed. 
-  
-
-Lemma add_red_var_unequal: 
-forall i u sigma j, program i -> program j -> i <> j -> 
-sf_red (App (App add (s_op2 (s_op2 sigma i) u)) (var j)) (App sigma (var j)).       
-Proof.
-intros. unfold_op;  unfold add at 1. 
-eapply transitive_red. eapply preserves_app_sf_red. eapply2 app_comb_red. 
-auto. 
-eapply transitive_red. eapply2 Y3_fix. 
-replace (app_comb (Y_k 3) add_fn) with add by auto. 
-unfold add_fn.
-eapply transitive_red. 
-eapply preserves_app_sf_red. 
-eapply2 star_opt_beta2.  auto. 
-unfold subst; rewrite ! subst_rec_preserves_extension. 
-eapply transitive_red. eapply2 extensions_by_matchfail.
-unfold var, var_fix, var_fn, app_comb; unfold_op. 
-eapply2 matchfail_compound_l. eapply2 matchfail_compound_r. 
-eapply2 matchfail_compound_l. eapply2 matchfail_compound_r.
-eapply2 matchfail_compound_r. 
-eapply2 matchfail_compound_l. eapply2 matchfail_compound_r. 
-eapply2 matchfail_compound_l. eapply2 matchfail_compound_r.
-eapply2 matchfail_compound_r. unfold Y_k, app_comb; unfold_op. 
-eapply2 matchfail_compound_l. eapply2 matchfail_compound_r. 
-eapply2 matchfail_compound_l. eapply2 matchfail_compound_r.
-eapply2 matchfail_compound_r. 
-eapply2 matchfail_compound_l. eapply2 matchfail_compound_r. 
-eapply2 matchfail_compound_l. eapply2 matchfail_compound_r.
-eapply2 matchfail_compound_r. unfold A_k, app_comb; unfold_op. 
-eapply2 matchfail_compound_l. eapply2 matchfail_compound_r. 
-eapply2 matchfail_compound_l. eapply2 matchfail_compound_l.
-eapply2 matchfail_op. unfold factorable. left; eauto. discriminate.
-(* 1 *)  
-eapply transitive_red. eapply2 extensions_by_matching.
-unfold var, var_fix, app_comb; unfold_op. 
-eapply2 match_app. eapply2 match_app. eapply2 match_app. 
-apply program_matching. 
-unfold program; split.  
-apply nf_compound. nf_out.
-apply nf_compound. nf_out.
-apply nf_compound.
-apply nf_compound. nf_out.
-apply nf_compound.
-apply nf_compound. nf_out.
-apply nf_compound. nf_out. auto. auto. auto. 
-apply nf_compound. nf_out. auto. auto. auto. auto. 
-nf_out. auto. auto. auto. auto. 
-eapply2 program_matching.  unfold program; auto. 
-unfold map, app, length, fold_left, subst. 
-unfold app_comb at 3 4 5 6; unfold_op. 
-unfold pattern_size; fold pattern_size.
-rewrite ! pattern_size_closed; auto.  unfold plus; fold plus. 
-rewrite ! subst_rec_app. rewrite ! (subst_rec_closed equal_comb). 2: auto. 
-rewrite ! subst_rec_preserves_snd_projection. 
-rewrite ! subst_rec_preserves_fst_projection. 
-repeat (rewrite subst_rec_ref at 1; insert_Ref_out). unfold lift. 
-rewrite ! lift_rec_lift_rec; try omega. unfold plus. 
-rewrite ! subst_rec_lift_rec; try omega.
-rewrite ! lift_rec_null.
-eapply transitive_red. eapply preserves_app_sf_red. eapply preserves_app_sf_red. 
-eapply preserves_app_sf_red. auto. 
-eapply transitive_red. eapply snd_preserves_sf_red. eapply2 fst_out.
-eapply2 snd_out.  
-eapply transitive_red. eapply snd_out. auto. 
-eapply preserves_app_sf_red.
-eapply fst_preserves_sf_red. eapply2 fst_out. auto. 
-eapply transitive_red. eapply preserves_app_sf_red. eapply preserves_app_sf_red.
-eapply2 unequal_programs. auto. 
-eapply transitive_red. eapply preserves_app_sf_red. eapply2 fst_out. auto. 
-auto. unfold_op.  
-eapply transitive_red. eapply preserves_app_sf_red. 
-eapply succ_red. eapply2 f_op_red. auto. auto. 
-eapply succ_red. eapply2 s_red. 
-eapply succ_red. eapply2 f_op_red.
-rewrite ! subst_rec_preserves_app_comb. 
-repeat (rewrite subst_rec_ref at 1; insert_Ref_out). 
-rewrite ! subst_rec_closed; auto.
-unfold lift; rewrite lift_rec_null; auto.  
-Qed.
-
-Lemma add_red_var_equal: 
-forall i u sigma, program i -> 
-sf_red (App (App add (s_op2 (s_op2 sigma i) u)) (var i)) u.       
-Proof.
-intros. unfold_op;  unfold add at 1. 
-eapply transitive_red. eapply preserves_app_sf_red. eapply2 app_comb_red. 
-auto. 
-eapply transitive_red. eapply2 Y3_fix. 
-replace (app_comb (Y_k 3) add_fn) with add by auto. 
-unfold add_fn.
-eapply transitive_red. 
-eapply preserves_app_sf_red. 
-eapply2 star_opt_beta2.  auto. 
-unfold subst; rewrite ! subst_rec_preserves_extension. 
-eapply transitive_red. eapply2 extensions_by_matchfail.
-unfold var, var_fix, var_fn, app_comb; unfold_op. 
-eapply2 matchfail_compound_l. eapply2 matchfail_compound_r. 
-eapply2 matchfail_compound_l. eapply2 matchfail_compound_r.
-eapply2 matchfail_compound_r. 
-eapply2 matchfail_compound_l. eapply2 matchfail_compound_r. 
-eapply2 matchfail_compound_l. eapply2 matchfail_compound_r.
-eapply2 matchfail_compound_r. unfold Y_k, app_comb; unfold_op. 
-eapply2 matchfail_compound_l. eapply2 matchfail_compound_r. 
-eapply2 matchfail_compound_l. eapply2 matchfail_compound_r.
-eapply2 matchfail_compound_r. 
-eapply2 matchfail_compound_l. eapply2 matchfail_compound_r. 
-eapply2 matchfail_compound_l. eapply2 matchfail_compound_r.
-eapply2 matchfail_compound_r. unfold A_k, app_comb; unfold_op. 
-eapply2 matchfail_compound_l. eapply2 matchfail_compound_r. 
-eapply2 matchfail_compound_l. eapply2 matchfail_compound_l.
-eapply2 matchfail_op. unfold factorable. left; eauto. discriminate.
-(* 1 *)  
-eapply transitive_red. eapply2 extensions_by_matching.
-unfold var, var_fix, app_comb; unfold_op. 
-eapply2 match_app. eapply2 match_app. eapply2 match_app. 
-eapply2 program_matching. 
-unfold program; split. nf_out. cbv; auto. 
-nf_out. auto. auto. 
-eapply2 program_matching.  unfold program; auto. 
-unfold map, app, length, fold_left, subst. 
-unfold app_comb at 3 4 5 6; unfold_op. 
-unfold pattern_size; fold pattern_size.
-rewrite ! pattern_size_closed; auto.  unfold plus; fold plus. 
-rewrite ! subst_rec_app. rewrite ! (subst_rec_closed equal_comb). 2: auto. 
-rewrite ! subst_rec_preserves_snd_projection. 
-rewrite ! subst_rec_preserves_fst_projection. 
-repeat (rewrite subst_rec_ref at 1; insert_Ref_out). unfold lift. 
-rewrite ! lift_rec_lift_rec; try omega. unfold plus. 
-rewrite ! subst_rec_lift_rec; try omega.
-rewrite ! lift_rec_null.
-eapply transitive_red. eapply preserves_app_sf_red. eapply preserves_app_sf_red. 
-eapply preserves_app_sf_red. auto. 
-eapply transitive_red. eapply snd_preserves_sf_red. eapply2 fst_out.
-eapply2 snd_out.  
-eapply transitive_red. eapply snd_out. auto. 
-eapply preserves_app_sf_red.
-eapply fst_preserves_sf_red. eapply2 fst_out. auto. 
-eapply transitive_red. eapply preserves_app_sf_red. eapply preserves_app_sf_red.
-eapply2 equal_programs. auto. 
-eapply transitive_red. eapply preserves_app_sf_red. eapply2 fst_out. auto. 
-auto. unfold_op.  
-eapply succ_red. eapply2 f_op_red. auto. 
-Qed.
-
-
-
-
-
-Lemma add_red_empty: 
-forall sigma x u, 
-sf_red (App (App add (s_op2 (s_op2 sigma x) u)) i_op) (App sigma i_op) .
-Proof.
-intros. unfold_op;  unfold add at 1. 
-eapply transitive_red. eapply preserves_app_sf_red. eapply2 app_comb_red. 
-auto. 
-eapply transitive_red. eapply2 Y3_fix. 
-replace (app_comb (Y_k 3) add_fn) with add by auto. 
-unfold add_fn.
-eapply transitive_red. 
-eapply preserves_app_sf_red. 
-eapply2 star_opt_beta2.  auto. 
-unfold subst; rewrite ! subst_rec_preserves_extension. 
-eapply transitive_red. eapply2 extensions_by_matchfail.
-unfold app_comb; unfold_op; auto. 
-eapply2 matchfail_compound_l. 
-eapply transitive_red. eapply2 extensions_by_matchfail.
-unfold app_comb; unfold_op; auto. 
-eapply2 matchfail_compound_l. 
-eapply transitive_red. eapply2 extensions_by_matchfail.
-unfold app_comb; unfold_op; auto. 
-eapply2 matchfail_compound_l. 
-eapply transitive_red. eapply2 extensions_by_matchfail.
-unfold app_comb; unfold_op; auto. 
-eapply2 matchfail_compound_l. 
-rewrite ! subst_rec_preserves_fst_projection. 
-unfold subst_rec; fold subst_rec. insert_Ref_out.
-unfold lift. rewrite lift_rec_lift_rec; try omega. unfold plus. 
-rewrite ! subst_rec_lift_rec; try omega.  
-rewrite ! lift_rec_null. 
-eapply transitive_red. eapply preserves_app_sf_red. 
-eapply fst_preserves_sf_red. eapply2 fst_out. auto. 
-eapply transitive_red. eapply preserves_app_sf_red. 
-eapply2 fst_out. auto. auto. 
-Qed. 
-
-
-Lemma add_red_abs : 
-forall xs sigma x t sigma2, 
-  sf_red (App (App add sigma2) (abs xs (s_op2 sigma x) t))
-         (abs xs (s_op2 (App (app_comb add sigma2) sigma) x) t)
-.
-Proof.
-intros. unfold_op;  unfold add at 1. 
-eapply transitive_red. eapply preserves_app_sf_red. eapply2 app_comb_red. 
-auto. 
-eapply transitive_red. eapply2 Y3_fix. 
-replace (app_comb (Y_k 3) add_fn) with add by auto. 
-unfold add_fn.
-eapply transitive_red. 
-eapply preserves_app_sf_red. 
-eapply2 star_opt_beta2.  auto. 
-unfold subst; rewrite ! subst_rec_preserves_extension. 
-eapply transitive_red. eapply2 extensions_by_matchfail.
-unfold abs, app_comb; unfold_op; auto. 
-eapply2 matchfail_compound_l. 
-eapply2 matchfail_compound_r. 
-eapply2 matchfail_compound_l. 
-eapply2 matchfail_compound_r. 
-eapply2 matchfail_compound_r. 
-eapply2 matchfail_compound_l. 
-eapply2 matchfail_compound_r. 
-eapply2 matchfail_compound_l. 
-eapply2 matchfail_compound_r. 
-eapply2 matchfail_compound_r. 
-eapply2 matchfail_compound_l. 
-eapply2 matchfail_compound_r. 
-eapply2 matchfail_compound_l. 
-eapply2 matchfail_compound_r. 
-eapply2 matchfail_compound_r.
-unfold Y_k, app_comb; unfold_op.  
-eapply2 matchfail_compound_l. 
-eapply2 matchfail_compound_r. 
-eapply2 matchfail_compound_l. 
-eapply2 matchfail_compound_r. 
-eapply2 matchfail_compound_r. 
-eapply2 matchfail_compound_l. 
-eapply2 matchfail_compound_r. 
-eapply2 matchfail_compound_l. 
-eapply2 matchfail_compound_r. 
-eapply2 matchfail_compound_r. 
-unfold A_k, app_comb; unfold_op.  
-eapply2 matchfail_compound_l. 
-eapply2 matchfail_compound_r. 
-eapply2 matchfail_compound_l. 
-eapply2 matchfail_compound_l. 
-eapply2 matchfail_op. unfold_op; 
-unfold factorable; split_all; left; eauto. discriminate.
-(* 1 *)  
-eapply  transitive_red. 
-eapply2 extensions_by_matchfail.
-unfold abs, app_comb; unfold_op; auto. 
-eapply2 matchfail_compound_l. 
-eapply2 matchfail_compound_r. 
-eapply2 matchfail_compound_l. 
-eapply2 matchfail_compound_r. 
-eapply2 matchfail_compound_r. 
-eapply2 matchfail_compound_l. 
-eapply2 matchfail_compound_r. 
-eapply2 matchfail_compound_l. 
-eapply2 matchfail_compound_r. 
-eapply2 matchfail_compound_r.
-unfold Y_k, app_comb; unfold_op.
-eapply2 matchfail_compound_l. 
-eapply2 matchfail_compound_r. 
-eapply2 matchfail_compound_l. 
-eapply2 matchfail_compound_r. 
-eapply2 matchfail_compound_r.
-eapply2 matchfail_compound_l. 
-eapply2 matchfail_compound_r. 
-eapply2 matchfail_compound_l. 
-eapply2 matchfail_compound_r. 
-eapply2 matchfail_compound_r. 
-unfold A_k, app_comb; unfold_op.  
-eapply2 matchfail_compound_l. 
-eapply2 matchfail_compound_r. 
-eapply2 matchfail_compound_l. 
-eapply2 matchfail_compound_l. 
-eapply2 matchfail_op. unfold_op; 
-unfold factorable; split_all; left; eauto. discriminate.
-(* 1 *)  
-eapply  transitive_red. 
-eapply2 extensions_by_matching.
-unfold abs, app_comb; unfold_op; auto. 
-do 20 eapply2 match_app. 
-eapply2 program_matching. 
-unfold map, app, length, fold_left, subst. 
-unfold subst. 
-rewrite ! subst_rec_preserves_app_comb. 
-rewrite ! (subst_rec_closed (Y_k _)). 
-unfold lift; rewrite ! lift_rec_null. 
-unfold app_comb at 5 6 7 8. 
-unfold_op; unfold pattern_size; fold pattern_size. unfold plus; fold plus. 
-rewrite pattern_size_closed. 
-2: auto.  2: auto. 2: auto.  2: auto. 2: auto.  2: auto. 2: auto.  
-unfold app_comb at 5 6 7 8 9 10 11 12 13 14 15 16 17 18 19 20
-21 22 23 24 25 26 27 28 29 30 31 32 33 34. 
-unfold_op; unfold pattern_size; fold pattern_size. 
-rewrite pattern_size_closed. unfold plus; fold plus. 
-repeat (rewrite subst_rec_ref; insert_Ref_out). 
-unfold subst_rec; fold subst_rec. insert_Ref_out. 
-repeat (rewrite subst_rec_ref; insert_Ref_out). 
-unfold lift; rewrite ! lift_rec_lift_rec; try omega. unfold plus; fold plus. 
-rewrite ! subst_rec_lift_rec; try omega.
-rewrite ! lift_rec_null. auto. 
-auto. 
-unfold app_comb; unfold_op; unfold pattern_size; fold pattern_size. 
-rewrite pattern_size_closed. unfold plus; fold plus. 
-rewrite Y_k_closed. omega. 
-auto.
-unfold app_comb; unfold_op; unfold pattern_size; fold pattern_size. 
-rewrite pattern_size_closed. unfold plus; fold plus. 
-rewrite Y_k_closed. omega. auto. 
-Qed.   
-
-Lemma size_add_fn : size add_fn = 46759. 
-Proof. 
-cbv; auto. Qed. 
 
 Lemma add_red_add: 
-forall i u sigma sigma2, 
-sf_red (App (App add sigma) (app_comb add (s_op2 (s_op2 sigma2 i) u)))
-        (app_comb add (s_op2 (s_op2 (App (app_comb add sigma) sigma2) i) 
-        (App (app_comb add sigma) u))). 
+forall sigma_x u sigma2 y v, 
+sf_red (App (App (App add sigma_x) u) (app_comb (app_comb add (s_op2 sigma2 y)) v))  
+        (app_comb (app_comb add (s_op2 (App (app_comb (app_comb add sigma_x) u) sigma2) y)) 
+        (App (app_comb (app_comb add sigma_x) u) v)). 
 Proof.
 intros. unfold_op;  unfold add at 1. 
-eapply transitive_red. eapply preserves_app_sf_red. eapply2 app_comb_red. 
-auto. 
-eapply transitive_red. eapply2 Y3_fix. 
-replace (app_comb (Y_k 3) add_fn) with add by auto. 
+eapply transitive_red. eapply preserves_app_sf_red. 
+eapply preserves_app_sf_red. eapply2 app_comb_red. 
+auto. auto. 
+eapply transitive_red. eapply2 Y4_fix. 
+replace (app_comb (Y_k 4) add_fn) with add by auto. 
 unfold add_fn.
 eapply transitive_red. 
 eapply preserves_app_sf_red. 
-eapply2 star_opt_beta2.  auto. 
+eapply2 star_opt_beta3.  auto. 
 unfold subst; rewrite ! subst_rec_preserves_extension. 
 (* not a tag *) 
 eapply transitive_red. apply extensions_by_matchfail.
@@ -823,6 +662,11 @@ eapply2 matchfail_compound_r.
 eapply2 matchfail_compound_l. 
 eapply2 matchfail_compound_r. 
 eapply2 matchfail_compound_r.
+eapply2 matchfail_compound_l. 
+eapply2 matchfail_compound_r. 
+eapply2 matchfail_compound_l. 
+eapply2 matchfail_compound_r. 
+eapply2 matchfail_compound_r. 
 unfold Y_k, app_comb; unfold_op. 
 eapply2 matchfail_compound_l. 
 eapply2 matchfail_compound_r. 
@@ -835,6 +679,17 @@ eapply2 matchfail_compound_l.
 eapply2 matchfail_compound_r. 
 eapply2 matchfail_compound_r. 
 unfold A_k, app_comb. unfold_op. 
+eapply2 matchfail_compound_l. 
+eapply2 matchfail_compound_r. 
+eapply2 matchfail_compound_r. 
+eapply2 matchfail_compound_r. 
+eapply2 matchfail_compound_r. 
+eapply2 matchfail_compound_l. 
+eapply2 matchfail_compound_r. 
+eapply2 matchfail_compound_r. 
+eapply2 matchfail_compound_r. 
+eapply2 matchfail_compound_r. 
+unfold app_comb; unfold_op; cbv. 
 eapply2 matchfail_compound_l. 
 eapply2 matchfail_compound_r. 
 eapply2 matchfail_compound_l. 
@@ -850,87 +705,174 @@ eapply2 matchfail_compound_r.
 eapply2 matchfail_compound_r. 
 eapply2 matchfail_compound_l. 
 eapply2 matchfail_compound_r.
-eapply2 matchfail_compound_r. 
-eapply2 program_matching. 
-unfold program; split; auto.  
-eapply2 matchfail_compound_r. 
-assert(matchfail var_fn add_fn \/ exists sigma, matching var_fn add_fn sigma).
-apply match_program. auto. 
-unfold program; split. apply add_fn_normal. 
-unfold add_fn. rewrite ! maxvar_star_opt. 
-repeat (rewrite maxvar_extension; rewrite ? maxvar_app; rewrite ? maxvar_app_comb).
-cbv.  auto.
-inversion H. auto. inversion H0. 
-
-assert(matchfail var_fn add_fn \/ exists sigma, matching var_fn add_fn sigma).
-apply match_program. apply var_fn_normal. split. 
-apply add_fn_normal.  
-unfold add_fn. rewrite ! maxvar_star_opt. 
-repeat (rewrite maxvar_extension; rewrite ? maxvar_app; rewrite ? maxvar_app_comb).
-cbv.  auto.
-inversion H2. auto. 
-inversion H3. 
-assert(add_fn = var_fn /\ x0 = nil) . 
-apply program_matching3. auto.  apply var_fn_closed.
-inversion H5. 
-assert(size add_fn = size var_fn) by congruence.  
-rewrite size_var_fn in H8; rewrite size_add_fn in H8. 
-discriminate. 
-(* 1 abs vs add *) 
-eapply transitive_red. eapply2 extensions_by_matchfail.
-unfold add, add_fn, app_comb; unfold_op; auto. 
 eapply2 matchfail_compound_l. 
 eapply2 matchfail_compound_r. 
-eapply2 matchfail_compound_l. 
 eapply2 matchfail_compound_r. 
+eapply2 matchfail_compound_l.
+unfold_op.  
 eapply2 matchfail_compound_r. 
 eapply2 matchfail_compound_l. 
 eapply2 matchfail_compound_r.
-eapply2 matchfail_compound_l. 
-eapply2 matchfail_compound_r. 
 eapply2 matchfail_compound_r.
-unfold Y_k, app_comb; unfold_op. 
 eapply2 matchfail_compound_l. 
+unfold_op. 
 eapply2 matchfail_compound_r. 
 eapply2 matchfail_compound_l. 
+eapply2 matchfail_compound_r. 
+eapply2 matchfail_compound_r. 
+eapply2 matchfail_compound_l. unfold_op. 
 eapply2 matchfail_compound_r.
-eapply2 matchfail_compound_r. 
-eapply2 matchfail_compound_l. 
-eapply2 matchfail_compound_r. 
-eapply2 matchfail_compound_l. 
-eapply2 matchfail_compound_r. 
-eapply2 matchfail_compound_r. 
-unfold A_k, app_comb. unfold_op. 
-eapply2 matchfail_compound_l. 
-eapply2 matchfail_compound_r. 
 eapply2 matchfail_compound_l. 
 eapply2 matchfail_compound_l. 
 eapply2 matchfail_op. unfold factorable. left; eauto. discriminate. 
+(* 1 *) 
 (* 1 add vs add *) 
 eapply transitive_red. eapply2 extensions_by_matching. 
 unfold app_comb; unfold_op. 
-repeat eapply2 match_app. 
+apply match_app. auto. auto. 
+apply match_app. auto. auto. auto. 
+apply match_app. auto. auto. 
+apply match_app. auto. auto. auto. 
+apply match_app. auto. auto. 
+eapply2 program_matching.  split; auto. 
+apply match_app. auto. auto. auto. 
+apply match_app. auto. auto. auto.  
+apply match_app. auto. auto. auto. 
+apply match_app. auto. auto. auto.  
+apply match_app. auto. auto. auto. 
+apply match_app. auto. auto. unfold_op. 
+apply match_app. auto. auto. auto. 
+eapply2 match_app. 
+eapply2 match_app. 
+eapply2 program_matching.  split; auto. 
+unfold_op; eapply2 program_matching. split; auto. 
+eapply2 match_app. 
+unfold_op; eapply2 program_matching. split; auto. 
+eapply2 match_app. 
+unfold_op; eapply2 program_matching. split; auto. 
+(* 1 *) 
 rewrite ! app_nil_r. 
 replace (length (nil : list SF)) with 0%nat by auto. 
 assert(forall A B f, map (f: A -> B) (nil: list A) = nil) by auto. 
 rewrite ! H. unfold app; fold app. 
-rewrite 40? map_lift0 at 1. 
+rewrite 10? map_lift0 at 1. 
 unfold length; fold length. 
 unfold map; fold map. 
-unfold fold_left. 
-replace  (0 +
-                     pattern_size
-                       (app_comb (Ref 3)
-                          (App (App (Op Sop) (App (App (Op Sop) (Ref 2)) (Ref 1))) (Ref 0))))%nat
-with 4%nat by (cbv; auto). 
+unfold fold_left.
 unfold subst; rewrite ! subst_rec_preserves_app_comb. 
-rewrite ! subst_rec_app. rewrite ! subst_rec_op. 
-rewrite ! subst_rec_preserves_app_comb.
+rewrite ! (subst_rec_closed (Y_k _)); try (rewrite Y_k_closed; omega).
+unfold app_comb at 4 5 6 7 8 9 10 11 12 13 14 15 16 17 18 19
+20 21 22 23 24 25 26 27 28 29 30 31 32 33 34 35 36 37 38. 
+unfold_op; unfold pattern_size; fold pattern_size. unfold plus; fold plus.
+rewrite ! pattern_size_closed; try (rewrite Y_k_closed; omega). 
+unfold plus; fold plus.   
+rewrite ! subst_rec_app. 
+repeat (rewrite subst_rec_ref; insert_Ref_out). 
+ unfold lift; rewrite ! lift_rec_lift_rec; try omega. unfold plus. 
+rewrite ! subst_rec_lift_rec; try omega. 
+rewrite ! lift_rec_null. rewrite ! subst_rec_op.  
+rewrite ! subst_rec_preserves_snd_projection. 
+rewrite ! subst_rec_preserves_fst_projection. 
 repeat (unfold subst_rec; fold subst_rec; insert_Ref_out). 
  unfold lift; rewrite ! lift_rec_lift_rec; try omega. unfold plus. 
 rewrite ! subst_rec_lift_rec; try omega. 
-rewrite ! lift_rec_null. auto. 
+rewrite ! lift_rec_null.
+(* 1 *) 
+eapply2 preserves_app_sf_red. unfold_op. 
+eapply2 preserves_app_sf_red. eapply2 preserves_app_sf_red. 
+eapply2 preserves_app_sf_red. eapply2 preserves_app_sf_red. 
+eapply2 preserves_app_sf_red. unfold_op. eapply2 preserves_app_sf_red. 
+eapply2 preserves_app_sf_red. eapply2 preserves_app_sf_red. 
+eapply2 preserves_app_sf_red. eapply2 preserves_app_sf_red. 
+eapply2 preserves_app_sf_red. eapply2 fst_out. eapply2 snd_out. 
 Qed. 
+
+
+Lemma add_red_empty: 
+forall sigma x u, 
+sf_red (App (App (App add (s_op2 sigma x)) u) i_op) (App sigma i_op) .
+Proof.
+intros. unfold_op;  unfold add at 1. 
+eapply transitive_red. eapply preserves_app_sf_red. 
+eapply preserves_app_sf_red. eapply2 app_comb_red. 
+auto. auto. 
+eapply transitive_red. eapply2 Y4_fix. 
+replace (app_comb (Y_k 4) add_fn) with add by auto. 
+unfold add_fn.
+eapply transitive_red. 
+eapply preserves_app_sf_red. 
+eapply2 star_opt_beta3.  auto. 
+unfold subst; rewrite ! subst_rec_preserves_extension. 
+eapply transitive_red. eapply2 extensions_by_matchfail.
+unfold app_comb; unfold_op; auto. 
+eapply2 matchfail_compound_l. 
+eapply transitive_red. eapply2 extensions_by_matchfail.
+unfold app_comb; unfold_op; auto. 
+eapply2 matchfail_compound_l. 
+eapply transitive_red. eapply2 extensions_by_matchfail.
+unfold app_comb; unfold_op; auto. 
+eapply2 matchfail_compound_l. 
+eapply transitive_red. eapply2 extensions_by_matchfail.
+unfold app_comb; unfold_op; auto. 
+eapply2 matchfail_compound_l. 
+rewrite ! subst_rec_preserves_fst_projection. 
+repeat (unfold subst_rec; fold subst_rec; insert_Ref_out).
+unfold lift. rewrite ! lift_rec_lift_rec; try omega. unfold plus. 
+rewrite ! subst_rec_lift_rec; try omega.  
+rewrite ! lift_rec_null. 
+eapply transitive_red. eapply preserves_app_sf_red. 
+eapply2 fst_out. auto. auto.  
+Qed. 
+
+
+
+(* delete 
+
+Definition add_fn := star_opt (star_opt (star_opt (star_opt 
+(* recursion argument, sigma, x and u *) 
+(* tag *) 
+(extension (app_comb(app_comb(app_comb (Y_k 3) (Ref 2)) (Ref 1)) (Ref 0)) 
+        (App (App (app_comb (app_comb (app_comb( Ref 6) (Ref 5)) (Ref 4)) (Ref 3)) (Ref 1))
+             (App (app_comb (app_comb (app_comb( Ref 6) (Ref 5)) (Ref 4)) (Ref 3)) (Ref 1)))
+(* var *) 
+(extension (app_comb (app_comb(Y_k 3) (Ref 1)) (Ref 0))  (* var y *) 
+                     (App (App (App (App equal_comb (Ref 0)) (Ref 3)) (* y = x *) 
+                               (Ref 2))  (* u *) 
+                          (App (Ref 2) (app_comb (app_comb(Y_k 3) (Ref 1)) (Ref 0))))
+                                          (* sigma (var y) *) 
+(* delete 
+(* abs *)
+(extension (app_comb (app_comb 
+(app_comb (app_comb(Y_k 4) (Ref 4)) (Ref 3)) (s_op2 (Ref 2) (Ref 1)))
+(Ref 0))
+           (app_comb (app_comb (app_comb 
+(app_comb (Y_k 4) (Ref 4)) (Ref 3))
+                                         (s_op2 (App (app_comb(Ref 6) (Ref 5)) (Ref 2)) (Ref 1)))
+                               (Ref 0))
+*) 
+
+
+(* add  *) 
+(* | Add i u sigma => App (App (Op Aop) add) (s_op2 (s_op2 (lambda_to_fieska sigma) (ref i)) (lambda_to_fieska u))
+*) 
+(extension (app_comb(app_comb(app_comb (app_comb (Y_k 5) (Ref 3)) (Ref 2)) (Ref 1)) (Ref 0))
+  (* add sigma2 x2 u *) 
+   (app_comb (app_comb(app_comb (app_comb (Y_k 5) (Ref 3))
+     (App (app_comb(app_comb(app_comb (Ref 7) (Ref 6)) (Ref 5)) (Ref 4)) (Ref 2)))
+       (Ref 1)) (Ref 0))
+(* abs = swap (add sigma2 x2) t *) 
+(extension (app_comb (app_comb (Ref 2) (Ref 1)) (Ref 0))
+            (app_comb (app_comb (Ref 2) 
+              (App (App (App (App (App (Y_k 5) (Ref 6)) (Ref 5)) (Ref 4)) (Ref 3)) (Ref 1))) (Ref 0))
+(* dummy case *) 
+i_op
+))))))).
+
+
+Lemma size_add_fn : size add_fn = 46759. 
+Proof. 
+cbv; auto. Qed. 
+
 
 (* 
 abs (A y ys) sigma_x t u  --> abs ys (S(S sigma_x u) y) t
@@ -942,5 +884,7 @@ applysub nil x ---> x
 *) 
 
 
+
+*) 
 
 
