Closure_calculus/README.md~
@@ -1,0 +1,16 @@
+# Closure_calculus
+
+The calculus is described in Closure_calculus.pdf.
+It generalizes the usual lambda abstractions to become *closures* 
+of the form 
+
+lambda x xs sigma t 
+
+where x xs is a non-empty sequence of bound variables, and sigma is an
+explicit substitution. 
+
+
+A key feature of this calculus is that reduction does not need to keep
+track of scopes in any way; no knowledge of free and bound variables,
+scopes or variable re-naming is required. This is a key step towards
+converting abstractions into combinations of operators.
